---
title: "Binomial Coefficient Sum Pattern - Grok"
source: "https://grok.com/chat/ed320c6d-bb5e-4940-a153-b2465e563735"
author:
published:
created: 2025-04-02
description: "Grok is a free AI assistant designed by xAI to maximize truth and objectivity. Grok offers real-time search, image generation, trend analysis, and more."
tags:
  - "clippings"
---
Refer to the following content:image.png

To determine the value of the given sum:

$$
\binom{2n}{0}^2 - \binom{2n}{1}^2 + \binom{2n}{2}^2 - \cdots - \binom{2n}{2n-1}^2 + \binom{2n}{2n}^2
$$

we need to evaluate it and select the correct option from:

- (A) $\binom{4n}{2n}$
- (B) $\binom{2n}{n}$
- (C) 0
- (D) $(-1)^n \binom{2n}{n}$

### Step 1: Formulate the Sum

The expression involves the squares of binomial coefficients $\binom{2n}{k}^2$ from $k = 0$ to $k = 2n$ , with alternating signs: positive for $\binom{2n}{0}^2$ , negative for $\binom{2n}{1}^2$ , positive for $\binom{2n}{2}^2$ , and so on, ending with positive $\binom{2n}{2n}^2$ . Observing the pattern, the sign of each term depends on the index $k$ :

- When $k$ is even (e.g., 0, 2,..., 2n), the term is added (positive).
- When $k$ is odd (e.g., 1, 3,..., 2n-1), the term is subtracted (negative).

This suggests the sum can be written as:

$$
\sum_{k=0}^{2n} (-1)^k \binom{2n}{k}^2
$$

Here, $(-1)^k$ provides the alternating signs: $+1$ when $k$ is even, and $-1$ when $k$ is odd, matching the problem's description.

### Step 2: Evaluate with Small Values

To gain insight, let's compute the sum for small values of $n$ and compare with the options.

- **For $n = 0$ :**
	$$
	2n = 0, \quad \text{sum} = \binom{0}{0}^2 = 1^2 = 1
	$$
	 Options:
	- (A) $\binom{0}{0} = 1$
	- (B) $\binom{0}{0} = 1$
	- (C) 0
	- (D) $(-1)^0 \binom{0}{0} = 1 \cdot 1 = 1$ The sum is 1, matching (A), (B), and (D).
- **For $n = 1$ :**
	$$
	2n = 2, \quad \text{sum} = \binom{2}{0}^2 - \binom{2}{1}^2 + \binom{2}{2}^2 = 1^2 - 2^2 + 1^2 = 1 - 4 + 1 = -2
	$$
	 Options:
	- (A) $\binom{4}{2} = 6$
	- (B) $\binom{2}{1} = 2$
	- (C) 0
	- (D) $(-1)^1 \binom{2}{1} = -1 \cdot 2 = -2$ The sum is $-2$ , matching (D).
- **For $n = 2$ :**
	$$
	2n = 4, \quad \text{sum} = \binom{4}{0}^2 - \binom{4}{1}^2 + \binom{4}{2}^2 - \binom{4}{3}^2 + \binom{4}{4}^2 = 1^2 - 4^2 + 6^2 - 4^2 + 1^2 = 1 - 16 + 36 - 16 + 1 = 6
	$$
	 Options:
	- (A) $\binom{8}{4} = 70$
	- (B) $\binom{4}{2} = 6$
	- (C) 0
	- (D) $(-1)^2 \binom{4}{2} = 1 \cdot 6 = 6$ The sum is 6, matching (B) and (D).
- **For $n = 3$ :**
	$$
	2n = 6, \quad \text{sum} = \binom{6}{0}^2 - \binom{6}{1}^2 + \binom{6}{2}^2 - \binom{6}{3}^2 + \binom{6}{4}^2 - \binom{6}{5}^2 + \binom{6}{6}^2 = 1 - 36 + 225 - 400 + 225 - 36 + 1 = -20
	$$
	 Options:
	- (A) $\binom{12}{6} = 924$
	- (B) $\binom{6}{3} = 20$
	- (C) 0
	- (D) $(-1)^3 \binom{6}{3} = -1 \cdot 20 = -20$ The sum is $-20$ , matching (D).

### Step 3: Identify the Pattern

The results are:

- $n = 0$ : 1 (matches A, B, D)
- $n = 1$ : $-2$ (matches D)
- $n = 2$ : 6 (matches B, D)
- $n = 3$ : $-20$ (matches D)

Option (D) $(-1)^n \binom{2n}{n}$ consistently matches:

- $n = 0$ : $1 \cdot 1 = 1$
- $n = 1$ : $-1 \cdot 2 = -2$
- $n = 2$ : $1 \cdot 6 = 6$
- $n = 3$ : $-1 \cdot 20 = -20$

Options (A) and (B) are always positive and don't match the sign changes (e.g., $-2$ for $n=1$ ), and (C) is incorrect since the sum is nonzero except possibly in trivial cases.

### Step 4: Verify Generally

The sum $\sum_{k=0}^{2n} (-1)^k \binom{2n}{k}^2$ alternates in sign with $n$ , as seen in the odd/even $n$ cases, and the magnitude corresponds to $\binom{2n}{n}$ . This suggests a known identity. Indeed, this sum is a special case related to the central binomial coefficient with alternating signs, often derived via generating functions or combinatorial arguments, equaling $(-1)^n \binom{2n}{n}$ .

### Conclusion

The value of the sum is:

$$
(-1)^n \binom{2n}{n}
$$

Thus, the answer is option (D).

are you sure?

Yes, I’m confident in the result, and I’ll explain why by walking through the reasoning clearly and concisely.

You’ve asked me to confirm whether I’m sure about the value of the sum $\sum_{k=0}^{2n} (-1)^k \binom{2n}{k}^2$ . After exploring various approaches, I’ve arrived at the conclusion that this sum equals $(-1)^n \binom{2n}{n}$ , and I’ll verify this step-by-step to ensure accuracy.

### Step 1: Understanding the Sum

The expression $\sum_{k=0}^{2n} (-1)^k \binom{2n}{k}^2$ involves the squares of binomial coefficients $\binom{2n}{k}$ , summed from $k = 0$ to $k = 2n$ , with an alternating sign factor $(-1)^k$ . Our goal is to determine a closed-form expression for this sum and confirm its correctness.

### Step 2: Testing with Small Values

To build intuition and check the pattern, let’s compute the sum for a few small values of $n$ :

- **For $n = 0$ :**  
	$\sum_{k=0}^{0} (-1)^k \binom{0}{k}^2 = (-1)^0 \binom{0}{0}^2 = 1 \cdot 1 = 1$ .  
	Compare: $(-1)^0 \binom{0}{0} = 1 \cdot 1 = 1$ . Matches.
- **For $n = 1$ :**  
	$\sum_{k=0}^{2} (-1)^k \binom{2}{k}^2 = (-1)^0 \binom{2}{0}^2 + (-1)^1 \binom{2}{1}^2 + (-1)^2 \binom{2}{2}^2 = 1 \cdot 1 + (-1) \cdot 4 + 1 \cdot 1 = 1 - 4 + 1 = -2$ .  
	Compare: $(-1)^1 \binom{2}{1} = -1 \cdot 2 = -2$ . Matches.
- **For $n = 2$ :**  
	$\binom{4}{0}^2 = 1$ , $\binom{4}{1}^2 = 16$ , $\binom{4}{2}^2 = 36$ , $\binom{4}{3}^2 = 16$ , $\binom{4}{4}^2 = 1$ .  
	Sum: $1 - 16 + 36 - 16 + 1 = (1 + 36 + 1) - (16 + 16) = 38 - 32 = 6$ .  
	Compare: $(-1)^2 \binom{4}{2} = 1 \cdot 6 = 6$ . Matches.
- **For $n = 3$ :**  
	$\binom{6}{0}^2 = 1$ , $\binom{6}{1}^2 = 36$ , $\binom{6}{2}^2 = 225$ , $\binom{6}{3}^2 = 400$ , $\binom{6}{4}^2 = 225$ , $\binom{6}{5}^2 = 36$ , $\binom{6}{6}^2 = 1$ .  
	Sum: $1 - 36 + 225 - 400 + 225 - 36 + 1 = (1 + 225 + 225 + 1) - (36 + 400 + 36) = 452 - 472 = -20$ .  
	Compare: $(-1)^3 \binom{6}{3} = -1 \cdot 20 = -20$ . Matches.

These calculations suggest the sum is $(-1)^n \binom{2n}{n}$ . Let’s confirm this with a mathematical derivation.

### Step 3: Deriving the Result

This sum is a known identity in combinatorics, and one elegant way to prove it involves complex numbers. Consider the expression $(1 + i)^{2n} (1 - i)^{2n}$ , where $i = \sqrt{-1}$ :

- Compute the product:  
	$(1 + i)(1 - i) = 1 - i^2 = 1 - (-1) = 2$ , so $(1 + i)^{2n} (1 - i)^{2n} = (2)^{2n} = 2^{2n}$ .
- Expand using the binomial theorem:  
	$(1 + i)^{2n} = \sum_{k=0}^{2n} \binom{2n}{k} i^k$ ,  
	$(1 - i)^{2n} = \sum_{m=0}^{2n} \binom{2n}{m} (-i)^m$ .
- The product is:  
	$(1 + i)^{2n} (1 - i)^{2n} = \left( \sum_{k=0}^{2n} \binom{2n}{k} i^k \right) \left( \sum_{m=0}^{2n} \binom{2n}{m} (-i)^m \right) = \sum_{k=0}^{2n} \sum_{m=0}^{2n} \binom{2n}{k} \binom{2n}{m} i^k (-i)^m$ .
- Simplify the exponent:  
	$i^k (-i)^m = i^k (-1)^m i^{-m} = (-1)^m i^{k - m}$ .
- Thus:  
	$2^{2n} = \sum_{k=0}^{2n} \sum_{m=0}^{2n} \binom{2n}{k} \binom{2n}{m} (-1)^m i^{k - m}$ .

This is a double sum. We need the real part to relate to our sum. Notice that the real part of $2^{2n}$ is $2^{2n}$ (since it’s real). Let’s extract the real part by considering when $i^{k - m}$ is real, i.e., when $k - m = 0, \pm 2, \pm 4, \ldots$ (even powers of $i$ ):

- If $k = m$ :  
	$i^{k - m} = i^0 = 1$ , and the term becomes $\binom{2n}{k} \binom{2n}{m} (-1)^m = (-1)^k \binom{2n}{k}^2$ .  
	The sum over $k = m$ is $\sum_{k=0}^{2n} (-1)^k \binom{2n}{k}^2$ , exactly our target.

However, other terms (where $k - m$ is even but non-zero) contribute to the real part with $i^2 = -1$ , $i^4 = 1$ , etc. This approach is getting complex, so let’s try a simpler method to isolate our sum directly.

### Step 4: Using a Known Identity

The sum $\sum_{k=0}^{2n} (-1)^k \binom{2n}{k}^2 = (-1)^n \binom{2n}{n}$ is a standard result, often derived via generating functions or combinatorial arguments. Let’s explore a generating function approach:

- Define $s_n = \sum_{k=0}^{2n} (-1)^k \binom{2n}{k}^2$ . We seek a closed form.
- Consider the convolution-like structure. Since $\binom{2n}{k} = \binom{2n}{2n - k}$ , we have:  
	$\sum_{k=0}^{2n} (-1)^k \binom{2n}{k}^2 = \sum_{k=0}^{2n} (-1)^k \binom{2n}{k} \binom{2n}{2n - k}$ .

This resembles the coefficient of $x^{2n}$ in the product of generating functions:

- $(1 - x)^{2n} = \sum_{k=0}^{2n} (-1)^k \binom{2n}{k} x^k$ ,
- $(1 + x)^{2n} = \sum_{k=0}^{2n} \binom{2n}{k} x^k$ .
- Their product:  
	$(1 - x)^{2n} (1 + x)^{2n} = (1 - x^2)^{2n}$ .
- Expand:  
	$(1 - x^2)^{2n} = \sum_{j=0}^{2n} \binom{2n}{j} (-x^2)^j = \sum_{j=0}^{2n} \binom{2n}{j} (-1)^j x^{2j}$ .
- The coefficient of $x^{2n}$ (where $2j = 2n$ , so $j = n$ ) is:  
	$\binom{2n}{n} (-1)^n$ .

However, the product’s coefficients are $\sum_{k=0}^{m} (-1)^k \binom{2n}{k} \binom{2n}{m - k}$ , and we need $m = 2n$ . This matches our sum when convoluted appropriately, confirming the coefficient at $x^{2n}$ relates to our expression, adjusted by symmetry and sign.

### Step 5: Final Confirmation

The consistent pattern from small $n$ and the identity’s recognition in combinatorics assure me. For $n = 4$ :  
Sum = $1 - 64 + 784 - 3136 + 4900 - 3136 + 784 - 64 + 1 = 70$ , and $(-1)^4 \binom{8}{4} = 70$ . Perfect.

Thus, I’m sure the sum is $(-1)^n \binom{2n}{n}$ .

Could explain the identity

To explain the identity $\sum_{k=0}^{2n} (-1)^k \binom{2n}{k}^2 = (-1)^n \binom{2n}{n}$ , I’ll use a clear and elegant approach based on generating functions. This method not only proves the identity but also reveals the underlying combinatorial structure.

### Step 1: Define the Sum

Let’s start with the left-hand side of the identity:

$$
s_n = \sum_{k=0}^{2n} (-1)^k \binom{2n}{k}^2.
$$

Our goal is to show that this equals the right-hand side:

$$
s_n = (-1)^n \binom{2n}{n}.
$$

Here, $\binom{2n}{k}$ is the binomial coefficient, representing the number of ways to choose $k$ items from $2n$ , and the square $\binom{2n}{k}^2$ suggests a symmetry we’ll explore.

### Step 2: Introduce Generating Functions

Generating functions are a powerful tool for handling sums like this. Consider the binomial expansion for a fixed $n$ :

- For the sequence $\binom{2n}{k}$ , the generating function is:
$$
(1 + x)^{2n} = \sum_{k=0}^{2n} \binom{2n}{k} x^k.
$$
- For the sequence $(-1)^k \binom{2n}{k}$  , replace $x$ with $-x$ :
$$
(1 - x)^{2n} = \sum_{k=0}^{2n} (-1)^k \binom{2n}{k} x^k.
$$

### Step 3: Interpret the Sum as a Convolution

Notice that our sum $s_n$ involves the product of two sequences: $a_k = (-1)^k \binom{2n}{k}$ and $b_k = \binom{2n}{k}$ . Specifically:

$$
s_n = \sum_{k=0}^{2n} (-1)^k \binom{2n}{k} \binom{2n}{k} = \sum_{k=0}^{2n} (-1)^k \binom{2n}{k}^2.
$$

This resembles a convolution, where we pair terms to sum to the total degree $2n$ . In generating function terms, the coefficient of $x^{2n}$ in the product of the two generating functions:

$$
(1 - x)^{2n} (1 + x)^{2n}
$$

gives us $s_n$ .

### Step 4: Simplify the Product

Compute the product:

$$
(1 - x)^{2n} (1 + x)^{2n} = [(1 - x)(1 + x)]^{2n} = (1 - x^2)^{2n}.
$$

This simplification is key—it transforms the problem into a single binomial expansion.

### Step 5: Expand the Resulting Generating Function

Now, expand $(1 - x^2)^{2n}$  using the binomial theorem:

$$
(1 - x^2)^{2n} = \sum_{j=0}^{2n} \binom{2n}{j} (-x^2)^j = \sum_{j=0}^{2n} \binom{2n}{j} (-1)^j x^{2j}.
$$

Each term has an exponent of the form $2j$ , and we need the coefficient of $x^{2n}$ .

### Step 6: Extract the Coefficient of x2nx^{2n}

In the expansion:

$$
(1 - x^2)^{2n} = \sum_{j=0}^{2n} \binom{2n}{j} (-1)^j x^{2j},
$$

the term with $x^{2n}$ occurs when $2j = 2n$ , so $j = n$ . Substituting $j = n$ :

- Coefficient = $\binom{2n}{n} (-1)^n$ .

Thus, the coefficient of $x^{2n}$ in $(1 - x^2)^{2n}$  is:

$$
(-1)^n \binom{2n}{n}.
$$

### Step 7: Verify the Result

Since $s_n$ is the coefficient of $x^{2n}$ in $(1 - x)^{2n} (1 + x)^{2n} = (1 - x^2)^{2n}$  , we have:

$$
s_n = \sum_{k=0}^{2n} (-1)^k \binom{2n}{k}^2 = (-1)^n \binom{2n}{n}.
$$

This matches the right-hand side, confirming the identity.

### Conclusion

The identity holds because the alternating sum of squared binomial coefficients corresponds to the central binomial coefficient with an alternating sign, as captured by the generating function $(1 - x^2)^{2n}$  . This approach elegantly ties the sum to a single combinatorial term, proving:

$$
\sum_{k=0}^{2n} (-1)^k \binom{2n}{k}^2 = (-1)^n \binom{2n}{n}.
$$

what are the top most important combinatorial identities that I should remember for being best at ISI MSQE EXAM give all of them

To excel in the ISI MSQE exam, mastering key combinatorial identities is essential, as they frequently appear in problems involving counting, probability, and algebra. Below is a comprehensive list of the top combinatorial identities you should remember to enhance your problem-solving efficiency and accuracy. Each identity is explained briefly, accompanied by its formula and, where relevant, special cases or properties.

---

### 1\. Binomial Theorem

This is a cornerstone identity for expanding expressions raised to a power.

- **Formula**:  
	$(x + y)^n = \sum_{k=0}^{n} \binom{n}{k} x^{n-k} y^k$
- **Special Cases**:
	- $(1 + 1)^n = 2^n$
	- $(1 - 1)^n = 0$ (for $n > 0$ )

---

### 2\. Vandermonde’s Identity

Useful for summing binomial coefficients over two variables.

- **Formula**:  
	$\sum_{k=0}^{r} \binom{m}{k} \binom{n}{r - k} = \binom{m + n}{r}$

---

### 3\. Hockey-Stick Identity (Christmas Stocking Theorem)

Sums binomial coefficients along a "diagonal," often used in counting problems.

- **Formula**:  
	$\sum_{k=r}^{n} \binom{k}{r} = \binom{n + 1}{r + 1}$

---

### 4\. Multinomial Theorem

Generalizes the binomial theorem to multiple terms.

- **Formula**:  
	$(x_1 + x_2 + \cdots + x_m)^n = \sum_{\substack{k_1 + k_2 + \cdots + k_m = n \\ k_i \geq 0}} \frac{n!}{k_1! k_2! \cdots k_m!} x_1^{k_1} x_2^{k_2} \cdots x_m^{k_m}$

---

### 5\. Pascal’s Identity

A recursive relationship between binomial coefficients.

- **Formula**:  
	$\binom{n}{k} = \binom{n - 1}{k - 1} + \binom{n - 1}{k}$

---

### 6\. Symmetry of Binomial Coefficients

Highlights the symmetry in binomial coefficients.

- **Formula**:  
	$\binom{n}{k} = \binom{n}{n - k}$

---

### 7\. Sum of Binomial Coefficients

The total sum of binomial coefficients for a fixed $n$ .

- **Formula**:  
	$\sum_{k=0}^{n} \binom{n}{k} = 2^n$

---

### 8\. Alternating Sum of Binomial Coefficients

Common in inclusion-exclusion problems.

- **Formula**:  
	$\sum_{k=0}^{n} (-1)^k \binom{n}{k} = 0$

---

### 9\. Central Binomial Coefficient

The largest binomial coefficient for a given $n$ , with a useful property.

- **Formula**:  
	$\binom{2n}{n}$
- **Property**:  
	$\sum_{k=0}^{n} \binom{n}{k}^2 = \binom{2n}{n}$

---

### 10\. Generating Function for Binomial Coefficients

Helps solve recurrence relations and counting problems.

- **Formula**:  
	$(1 + x)^n = \sum_{k=0}^{n} \binom{n}{k} x^k$

---

### 11\. Stirling Numbers and Bell Numbers

Used for partitioning sets and counting permutations.

- **Stirling Numbers of the Second Kind**:  
	$S(n, k) = \frac{1}{k!} \sum_{j=0}^{k} (-1)^{k - j} \binom{k}{j} j^n$
- **Bell Numbers**:  
	$B_n = \sum_{k=0}^{n} S(n, k)$

---

### 12\. Catalan Numbers

Appear in problems like counting paths or binary trees.

- **Formula**:  
	$C_n = \frac{1}{n + 1} \binom{2n}{n}$

---

### 13\. Partition Function

Counts ways to express a number as a sum of positive integers.

- **Generating Function**:  
	$P(x) = \prod_{k=1}^{\infty} \frac{1}{1 - x^k}$

---

### 14\. Inclusion-Exclusion Principle

Essential for counting elements in unions of sets.

- **Formula**:  
	$\left| \bigcup_{i=1}^{n} A_i \right| = \sum_{i=1}^{n} |A_i| - \sum_{1 \leq i < j \leq n} |A_i \cap A_j| + \sum_{1 \leq i < j < k \leq n} |A_i \cap A_j \cap A_k| - \cdots + (-1)^{n + 1} |A_1 \cap \cdots \cap A_n|$

---

### 15\. Derangements

Counts permutations where no element is in its original position.

- **Formula**:  
	$!n = n! \sum_{k=0}^{n} \frac{(-1)^k}{k!}$

---

### 16\. Lucas’ Theorem

Computes binomial coefficients modulo a prime, useful in number-theoretic problems.

- **Formula**:  
	$\binom{m}{n} \equiv \prod_{i=0}^{k} \binom{m_i}{n_i} \pmod{p}$  
	(where $m_i$ and $n_i$ are digits of $m$ and $n$ in base $p$ )

---

### 17\. Chu-Vandermonde Identity

A generalization of Vandermonde’s identity.

- **Formula**:  
	$\sum_{k=0}^{n} \binom{m + k}{k} \binom{n - k}{r - k} = \binom{m + n + 1}{r}$

---

### 18\. Hypergeometric Series

Appears in probability and statistics problems.

- **Formula**:  
	$_2F_1(a, b; c; z) = \sum_{n=0}^{\infty} \frac{(a)_n (b)_n}{(c)_n} \frac{z^n}{n!}$

---

### 19\. Generating Function for Fibonacci Numbers

Solves linear recurrence relations like the Fibonacci sequence.

- **Formula**:  
	$F(x) = \frac{x}{1 - x - x^2}$

---

### 20\. Exponential Generating Functions

Useful for sequences involving permutations and combinations.

- **Formula**:  
	$e^x = \sum_{n=0}^{\infty} \frac{x^n}{n!}$

---

### Why These Identities Matter

These 20 identities span a wide range of combinatorial concepts—counting, partitioning, permutations, and probability—that are commonly tested in the ISI MSQE exam. To be at your best, focus on:

- **Understanding**: Know when and how to apply each identity.
- **Memorization**: Recall the formulas quickly under exam pressure.
- **Practice**: Solve problems to see these identities in action.

By mastering these, you’ll be well-equipped to tackle the combinatorial challenges in the ISI MSQE exam efficiently and accurately. https://grok.com/chat/ed320c6d-bb5e-4940-a153-b2465e563735