---
title: "Coefficient of \ t^3 \ in Expansion - Grok"
source: "https://grok.com/chat/3c8d2b53-a240-4e68-a380-62acc408cc4d"
author:
published:
created: 2025-04-02
description: "Grok is a free AI assistant designed by xAI to maximize truth and objectivity. Grok offers real-time search, image generation, trend analysis, and more."
tags:
  - "clippings"
---
Refer to the following content:image.png

To find the coefficient of $t^3$  in the expansion of $\left(\frac{1 - t^6}{1 - t}\right)^3$ , let’s proceed step-by-step.

First, simplify the expression inside the parentheses. Notice that:

$$
\frac{1 - t^6}{1 - t}
$$

can be rewritten by recognizing that $1 - t^6$  is a difference of powers. We can factor it as:

$$
1 - t^6 = (1 - t)(1 + t + t^2 + t^3 + t^4 + t^5)
$$

This is a geometric series sum, where:

$$
1 + t + t^2 + t^3 + t^4 + t^5 = \frac{1 - t^6}{1 - t}
$$

Thus:

$$
\frac{1 - t^6}{1 - t} = 1 + t + t^2 + t^3 + t^4 + t^5
$$

So the original expression becomes:

$$
\left(\frac{1 - t^6}{1 - t}\right)^3 = \left(1 + t + t^2 + t^3 + t^4 + t^5\right)^3
$$

We need the coefficient of $t^3$  in the expansion of:

$$
\left(1 + t + t^2 + t^3 + t^4 + t^5\right)^3
$$

This is a polynomial raised to the third power, and each term in the polynomial $1 + t + t^2 + t^3 + t^4 + t^5$  has a coefficient of 1. Expanding this directly could be tedious, so let’s consider the terms that contribute to $t^3$  when multiplying three such polynomials.

Each factor is $1 + t + t^2 + t^3 + t^4 + t^5$  , and we select one term from each factor such that the exponents sum to 3. Let the exponents chosen from the three factors be $a$  , $b$  , and $c$  , where $0 \leq a, b, c \leq 5$  , and we need:

$$
a + b + c = 3
$$

Since each term $t^k$  has a coefficient of 1, the coefficient of $t^3$  is the number of ways to choose $a$  , $b$  , and $c$  (non-negative integers) satisfying this equation, with the constraint $0 \leq a, b, c \leq 5$  . Because the target exponent 3 is less than the maximum exponent 5, all solutions will naturally satisfy $a, b, c \leq 3 \leq 5$  , so the upper bound doesn’t restrict us here.

This is a classic “stars and bars” problem: find the number of non-negative integer solutions to $a + b + c = 3$  . The number of solutions is given by:

$$
\binom{n + r - 1}{r - 1}
$$

where $n = 3$  (the sum) and $r = 3$  (the number of variables):

$$
\binom{3 + 3 - 1}{3 - 1} = \binom{5}{2}
$$

Calculate:

$$
\binom{5}{2} = \frac{5 \cdot 4}{2} = 10
$$

So, there are 10 solutions. Let’s list them to confirm:

- $(3, 0, 0)$  , $(0, 3, 0)$  , $(0, 0, 3)$  → 3 ways
- $(2, 1, 0)$  , $(2, 0, 1)$  , $(1, 2, 0)$  , $(0, 2, 1)$  , $(1, 0, 2)$  , $(0, 1, 2)$  → 6 ways
- $(1, 1, 1)$  → 1 way

Total: $3 + 6 + 1 = 10$  . Each solution contributes a term $t^a \cdot t^b \cdot t^c = t^{a+b+c} = t^3$  with coefficient $1 \cdot 1 \cdot 1 = 1$  , so the coefficient of $t^3$  is 10.

Alternatively, consider the generating function approach. Since:

$$
\left(\frac{1 - t^6}{1 - t}\right)^3 = \frac{(1 - t^6)^3}{(1 - t)^3}
$$

Expand the numerator:

$$
(1 - t^6)^3 = 1 - 3t^6 + 3t^{12} - t^{18}
$$

For the denominator, use the series expansion of $\frac{1}{(1 - t)^3}$  :

$$
\frac{1}{(1 - t)^3} = \sum_{k=0}^{\infty} \binom{k + 2}{2} t^k
$$

where $\binom{k + 2}{2} = \frac{(k + 2)(k + 1)}{2}$  . The full expression is:

$$
(1 - 3t^6 + 3t^{12} - t^{18}) \cdot \sum_{k=0}^{\infty} \binom{k + 2}{2} t^k
$$

The coefficient of $t^3$  comes from terms where the exponents add to 3:

- From $1 \cdot t^3$  : coefficient is $\binom{3 + 2}{2} = \binom{5}{2} = 10$
- From $-3t^6 \cdot t^{3-6} = -3t^6 \cdot t^{-3}$  : no $t^{-3}$  in the series (exponents are non-negative)
- From $3t^{12} \cdot t^{3-12} = 3t^{12} \cdot t^{-9}$  : no $t^{-9}$
- From $-t^{18} \cdot t^{3-18} = -t^{18} \cdot t^{-15}$  : no $t^{-15}$

Only the first term contributes, giving a coefficient of 10.

Both methods agree, and since $t^3$  has exponent 3, and the polynomial $1 + t + t^2 + t^3 + t^4 + t^5$  includes terms up to $t^5$  , the coefficient matches that of $\left( \frac{1}{1 - t} \right)^3$  up to $t^3$  , adjusted by the truncation at $t^6$  , but unaffected here.

Thus, the coefficient of $t^3$  is 10, matching option (A).

**Answer: 10**

I could not undertand the talk about factors and choosing a, b, c

I understand that the discussion about factors and choosing $a$ , $b$ , and $c$ might have been confusing. Let me explain it clearly and simply, step by step, so you can follow how we find the coefficient of $t^3$ in the expansion of $\left(\frac{1 - t^6}{1 - t}\right)^3$ .

### Step 1: Simplify the Expression

First, let’s look at the expression inside the parentheses: $\frac{1 - t^6}{1 - t}$ . This looks like a geometric series. You might recall that:

$$
1 + t + t^2 + t^3 + t^4 + t^5 = \frac{1 - t^6}{1 - t}
$$

This is because the formula for the sum of a geometric series is $\frac{1 - r^n}{1 - r}$ , where $r = t$ and $n = 6$ , giving us terms from $t^0 = 1$ up to $t^5$ . So, the original expression becomes:

$$
\left(\frac{1 - t^6}{1 - t}\right)^3 = \left(1 + t + t^2 + t^3 + t^4 + t^5\right)^3
$$

Our goal is to expand this and find the coefficient of $t^3$ .

### Step 2: Understand the Expansion

We need to expand $\left(1 + t + t^2 + t^3 + t^4 + t^5\right)^3$ . This means we’re multiplying three identical polynomials:

$$
(1 + t + t^2 + t^3 + t^4 + t^5) \times (1 + t + t^2 + t^3 + t^4 + t^5) \times (1 + t + t^2 + t^3 + t^4 + t^5)
$$

Each polynomial has the terms $1, t, t^2, t^3, t^4, t^5$ , which we can think of as $t^0, t^1, t^2, t^3, t^4, t^5$ , where the exponents are 0, 1, 2, 3, 4, and 5, and each term has a coefficient of 1.

When we multiply these together, we pick one term from each polynomial and multiply them. The result is a term of the form $t^a \cdot t^b \cdot t^c = t^{a + b + c}$ , where:

- $a$ is the exponent from the first polynomial,
- $b$ is the exponent from the second polynomial,
- $c$ is the exponent from the third polynomial,
- and each $a, b, c$ can be any number from 0 to 5 (since the terms go from $t^0$ to $t^5$ ).

The coefficient of that resulting term is the product of the coefficients of the chosen terms, which is $1 \times 1 \times 1 = 1$ .

### Step 3: Find Terms That Give t3t^3

Since we want the coefficient of $t^3$ , we need the total exponent to be 3:

$$
a + b + c = 3
$$

Also, because each polynomial only has terms up to $t^5$ , we have:

$$
0 \leq a \leq 5, \quad 0 \leq b \leq 5, \quad 0 \leq c \leq 5
$$

We need to find all possible ways to choose $a, b, c$ as non-negative integers (0, 1, 2, 3, 4, or 5) that add up to 3. Then, the coefficient of $t^3$ will be the number of such combinations, because each combination contributes a $t^3$ term with a coefficient of 1.

### Step 4: Count the Combinations

Let’s list all the ways that $a + b + c = 3$ with $a, b, c \geq 0$ . Since the sum is only 3, and 3 is less than 5, we won’t even reach the upper limit of 5 unless one number takes all the value (like 3), which is fine because 3 is still less than or equal to 5. Here are all the possibilities:

- **One number is 3, the others are 0:**
	- $(3, 0, 0)$ : $3 + 0 + 0 = 3$
	- $(0, 3, 0)$ : $0 + 3 + 0 = 3$
	- $(0, 0, 3)$ : $0 + 0 + 3 = 3$
	- That’s 3 ways.
- **One number is 2, another is 1, one is 0:**
	- $(2, 1, 0)$ : $2 + 1 + 0 = 3$
	- $(2, 0, 1)$ : $2 + 0 + 1 = 3$
	- $(1, 2, 0)$ : $1 + 2 + 0 = 3$
	- $(1, 0, 2)$ : $1 + 0 + 2 = 3$
	- $(0, 2, 1)$ : $0 + 2 + 1 = 3$
	- $(0, 1, 2)$ : $0 + 1 + 2 = 3$
	- That’s 6 ways.
- **All three numbers are 1:**
	- $(1, 1, 1)$ : $1 + 1 + 1 = 3$
	- That’s 1 way.

Total number of ways = $3 + 6 + 1 = 10$ .

Each of these combinations gives $t^3$ (e.g., $t^3 \cdot t^0 \cdot t^0 = t^3$ , $t^2 \cdot t^1 \cdot t^0 = t^3$ , $t^1 \cdot t^1 \cdot t^1 = t^3$ ), and since each term we picked has a coefficient of 1, each combination adds 1 to the coefficient of $t^3$ .

### Step 5: Why This Makes Sense

You might wonder why we’re just counting combinations. Think of it like this: every time we multiply the polynomials, we’re building terms by adding their exponents. The coefficient of $t^3$ is how many times $t^3$ appears in the result, which depends on how many ways we can select exponents that sum to 3 from the available terms.

Since the highest exponent in each polynomial is 5, and we’re only looking for $t^3$ , all possible ways to reach 3 are included (the largest $a, b,$ or $c$ we need is 3, which is less than 5), so there’s no restriction cutting off our combinations.

### Step 6: Verify with a Simpler Example

To feel confident, imagine a smaller case, like $(1 + t + t^2)^3$ , and find the coefficient of $t^3$ . Here, exponents are 0, 1, 2:

- $(1, 1, 1)$ : $1 + 1 + 1 = 3$
- $(2, 1, 0)$ and permutations: $(2, 1, 0)$ , $(2, 0, 1)$ , $(1, 2, 0)$ , $(1, 0, 2)$ , $(0, 2, 1)$ , $(0, 1, 2)$

That’s $1 + 6 = 7$ ways, which makes sense for that case. For our problem, with terms up to $t^5$ , we get more combinations (10), which fits because we have more terms to choose from.

### Final Answer

The coefficient of $t^3$ is the number of ways to choose $a, b, c$ that sum to 3, which is 10. So, the coefficient is 10. I hope this clears up the process—let me know if you need more help!

how much more

I need more context to provide an accurate answer to your question, "how much more." This phrase typically involves comparing two quantities, such as cost, time, or amount, but I’m not sure what you’re referring to. Could you please specify what you’re comparing? For example:

- Are you asking about the difference in price between two items?
- Do you want to know how much more time something takes compared to another option?
- Are you looking for the increase in a value, like quantity or distance?

The more details you provide, the better I can assist you with a precise and relevant answer. Please let me know!

try to illustrate more explain every detail

To find the coefficient of $t^3$  in the expansion of $\left( \frac{1 - t^6}{1 - t} \right)^3$  , we need to determine what this expression represents as a polynomial and then identify the coefficient of the $t^3$  term. Let’s break this down step by step, explaining every detail as clearly as possible.

---

### Step 1: Simplify the Expression Inside the Parentheses

We start with the expression inside the parentheses: $\frac{1 - t^6}{1 - t}$  . Our goal is to rewrite this in a form that’s easier to work with when raised to the third power.

- **Numerator**: The numerator is $1 - t^6$  . This looks like a difference, and we might recognize it as related to a geometric series or factoring. For now, let’s hold off on factoring and consider what happens when we divide it by the denominator.
- **Denominator**: The denominator is $1 - t$  . This resembles the denominator of a geometric series sum, suggesting that $\frac{1}{1 - t}$  could be expanded as a series, but here it’s dividing $1 - t^6$  .
- **Geometric Series Insight**: Recall the formula for the sum of a geometric series:
	$$
	1 + t + t^2 + t^3 + t^4 + t^5 + \cdots = \frac{1}{1 - t}
	$$
	This is an infinite series, valid for $|t| < 1$  , but notice that if we truncate it after $t^5$  (6 terms, from $t^0$  to $t^5$  ), we get:
	$$
	1 + t + t^2 + t^3 + t^4 + t^5 = \frac{1 - t^6}{1 - t}
	$$
	Let’s verify this:
	- Multiply both sides by $1 - t$  :
		$$
		(1 - t)(1 + t + t^2 + t^3 + t^4 + t^5)
		$$
		- Distribute:
			$$
			= 1 + t + t^2 + t^3 + t^4 + t^5 - t - t^2 - t^3 - t^4 - t^5 - t^6
			$$
		- Combine like terms:
			- $1$  (no other constant term)
			- $t - t = 0$
			- $t^2 - t^2 = 0$
			- $t^3 - t^3 = 0$
			- $t^4 - t^4 = 0$
			- $t^5 - t^5 = 0$
			- $-t^6$
		- Result: $1 - t^6$  , which matches the numerator!
	So:
	$$
	\frac{1 - t^6}{1 - t} = 1 + t + t^2 + t^3 + t^4 + t^5
	$$
	This is a polynomial with terms from $t^0$  to $t^5$  , each with a coefficient of 1.
- **Result**: The original expression becomes:
	$$
	\left( \frac{1 - t^6}{1 - t} \right)^3 = \left( 1 + t + t^2 + t^3 + t^4 + t^5 \right)^3
	$$

---

### Step 2: Interpret the Expansion

Now we need to expand:

$$
\left( 1 + t + t^2 + t^3 + t^4 + t^5 \right)^3
$$

This means:

$$
(1 + t + t^2 + t^3 + t^4 + t^5) \times (1 + t + t^2 + t^3 + t^4 + t^5) \times (1 + t + t^2 + t^3 + t^4 + t^5)
$$
- Each factor is a polynomial with 6 terms: $1, t, t^2, t^3, t^4, t^5$  .
- To expand this, we pick one term from each of the three factors, multiply them, and sum all such products.
- The exponent of the resulting term is the sum of the exponents from each factor, and the coefficient depends on how many ways we can achieve that sum.

For example:

- Pick $1$  (i.e., $t^0$  ) from all three: $t^0 \cdot t^0 \cdot t^0 = t^0$  , coefficient 1.
- Pick $t^2, t^1, t^0$  : $t^2 \cdot t^1 \cdot t^0 = t^{2+1+0} = t^3$  , coefficient 1 for this specific combination.

Since each term in $1 + t + t^2 + t^3 + t^4 + t^5$  has a coefficient of 1, the coefficient of $t^n$  in the expansion is the number of ways to choose terms whose exponents sum to $n$  .

---

### Step 3: Focus on the t3 t^3 Term

We want the coefficient of $t^3$  . For a term to be $t^3$  , the exponents of the terms we pick from each factor must add up to 3. Let:

- $a$  be the exponent from the first factor,
- $b$  be the exponent from the second factor,
- $c$  be the exponent from the third factor.

Then we need:

$$
a + b + c = 3
$$

where $a, b, c$  can be any exponent available in the polynomial, i.e., $\{0, 1, 2, 3, 4, 5\}$  , because the terms are $t^0, t^1, t^2, t^3, t^4, t^5$  .

- **Constraints**: Since we’re looking for $t^3$  , and the maximum exponent in each polynomial is 5, we should check if the upper limit affects us. The largest single exponent contributing to 3 would be 3 (e.g., $3 + 0 + 0$  ), which is ≤ 5, so all possible combinations up to 3 are within bounds.
- **Problem Type**: This is a combinatorics problem: find the number of non-negative integer solutions to $a + b + c = 3$  where $a, b, c \geq 0$  , and technically $a, b, c \leq 5$  , but since 3 is small, the upper bound won’t restrict us here.

---

### Step 4: Calculate the Number of Solutions

The number of non-negative integer solutions to $x_1 + x_2 + \cdots + x_r = n$  is given by the "stars and bars" theorem:

$$
\binom{n + r - 1}{r - 1}
$$
- $n = 3$  (the sum we want),
- $r = 3$  (three variables: $a, b, c$  ).

So:

$$
\binom{3 + 3 - 1}{3 - 1} = \binom{5}{2}
$$

Compute:

$$
\binom{5}{2} = \frac{5!}{2! (5 - 2)!} = \frac{5 \times 4 \times 3!}{2 \times 1 \times 3!} = \frac{5 \times 4}{2} = \frac{20}{2} = 10
$$

So, there are 10 solutions.

---

### Step 5: List All Combinations

Let’s list all ways $a + b + c = 3$  with $a, b, c \geq 0$  to confirm:

1. **$a = 3, b = 0, c = 0$** :
	- $(3, 0, 0)$
	- $(0, 3, 0)$
	- $(0, 0, 3)$
	- 3 ways.
2. **$a = 2, b = 1, c = 0$** :
	- $(2, 1, 0)$
	- $(2, 0, 1)$
	- $(1, 2, 0)$
	- $(1, 0, 2)$
	- $(0, 2, 1)$
	- $(0, 1, 2)$
	- 6 ways.
3. **$a = 1, b = 1, c = 1$** :
	- $(1, 1, 1)$
	- 1 way.

Total: $3 + 6 + 1 = 10$  .

Each combination corresponds to picking terms:

- $(3, 0, 0)$  : $t^3 \cdot t^0 \cdot t^0 = t^3$  ,
- $(2, 1, 0)$  : $t^2 \cdot t^1 \cdot t^0 = t^3$  ,
- $(1, 1, 1)$  : $t^1 \cdot t^1 \cdot t^1 = t^3$  .

Since each term’s coefficient is 1, each combination adds 1 to the coefficient of $t^3$  , totaling 10.

---

### Step 6: Verify with an Alternative Method

Let’s try expanding $\left( \frac{1 - t^6}{1 - t} \right)^3 = \frac{(1 - t^6)^3}{(1 - t)^3}$  :

- **Numerator**: $(1 - t^6)^3$  :
	$$
	(1 - t^6)^3 = 1 - 3 t^6 + 3 t^{12} - t^{18}
	$$
	(Using binomial expansion: $(a - b)^3 = a^3 - 3a^2b + 3ab^2 - b^3$  , where $a = 1, b = t^6$  ).
- **Denominator**: $\frac{1}{(1 - t)^3}$  : The series is:
	$$
	\frac{1}{(1 - t)^3} = \sum_{k=0}^{\infty} \binom{k + 2}{2} t^k
	$$
	- Coefficient of $t^3$  : $\binom{3 + 2}{2} = \binom{5}{2} = 10$  .
- **Multiply**:
	$$
	(1 - 3 t^6 + 3 t^{12} - t^{18}) \times \sum_{k=0}^{\infty} \binom{k + 2}{2} t^k
	$$
	For $t^3$  :
	- $1 \times t^3$  : coefficient $\binom{5}{2} = 10$  ,
	- $-3 t^6 \times t^{3-6} = -3 t^{-3}$  : no such term (exponent negative),
	- $3 t^{12} \times t^{3-12} = 3 t^{-9}$  : no such term,
	- $-t^{18} \times t^{3-18} = -t^{-15}$  : no such term.
	Only the first term contributes: coefficient is 10.

---

### Final Answer

The coefficient of $t^3$  in the expansion of $\left( \frac{1 - t^6}{1 - t} \right)^3$  is 10, confirmed by both methods. https://grok.com/chat/3c8d2b53-a240-4e68-a380-62acc408cc4d