---
title: "Utility Maximization Problem Solution - Grok"
source: "https://grok.com/chat/5ed2d142-4d00-49a0-9b5e-6cfd0247a8dc"
author:
published:
created: 2025-03-28
description: "Grok is a free AI assistant designed by xAI to maximize truth and objectivity. Grok offers real-time search, image generation, trend analysis, and more."
tags:
  - "clippings"
---
Refer to the following content:image.png

To solve this utility maximization problem, we need to determine the equilibrium quantities $(x^*, y^*)$  that maximize the utility function subject to the budget constraint and then identify which of the given statements must always be true.

### Step 1: Understand the Problem

We are given:

- **Utility function**: $u(x, y) = A\sqrt{xy}$  , where $A > 0$  , and $x \geq 0$  , $y \geq 0$  are the amounts of goods $X$  and $Y$  consumed.
- **Budget constraint**: $P_X x + P_Y y \leq M$  , where $M > 0$  is the consumer's income, and $P_X$  and $P_Y$  are the prices of goods $X$  and $Y$  .
- **Price condition**: $P_X = P_Y > 1$  .
- **Objective**: Find $(x^*, y^*)$  that maximizes utility and determine which of the following holds:
	- (A) $x^* > y^*$
	- (B) $x^* = y^*$
	- (C) $x^* < y^*$
	- (D) $x^* + y^* = M$

Since $P_X = P_Y$  , let’s denote the common price as $P$  , where $P > 1$  . The budget constraint simplifies to:

$$
P x + P y \leq M
$$

or equivalently:

$$
P (x + y) \leq M
$$

### Step 2: Hypothesize Full Expenditure

The utility function $u(x, y) = A\sqrt{xy}$  is increasing in both $x$  and $y$  for $x, y > 0$  (since $\sqrt{xy}$  increases as $x$  or $y$  increases, and $A > 0$  ). This suggests that the consumer will maximize utility by spending all available income, making the budget constraint hold with equality:

$$
P (x^* + y^*) = M
$$

This implies:

$$
x^* + y^* = \frac{M}{P}
$$

Since $P > 1$  and $M > 0$  , we note that:

$$
\frac{M}{P} < M
$$

This observation will help us evaluate option (D) later.

### Step 3: Set Up the Optimization

To find $(x^*, y^*)$  , we maximize:

$$
u(x, y) = A \sqrt{xy}
$$

subject to:

$$
P x + P y = M
$$

with $x \geq 0$  , $y \geq 0$  .

#### Substitution Method

Solve the budget constraint for $y$  :

$$
P y = M - P x \quad \Rightarrow \quad y = \frac{M - P x}{P}
$$

Substitute into the utility function:

$$
u(x) = A \sqrt{x \cdot \frac{M - P x}{P}} = A \sqrt{\frac{x (M - P x)}{P}}
$$

Since $A > 0$  and $P > 0$  , we can maximize the expression under the square root, or equivalently, maximize $u(x)^2$  to simplify differentiation (the square is a monotonic transformation for positive values):

$$
u(x)^2 = A^2 \cdot \frac{x (M - P x)}{P}
$$

Define:

$$
f(x) = \frac{x (M - P x)}{P} = \frac{M x - P x^2}{P}
$$

Maximize $f(x)$  with respect to $x$  , where $0 \leq x \leq \frac{M}{P}$  (since $y \geq 0 \Rightarrow M - P x \geq 0$  ).

#### Take the Derivative

$$
f'(x) = \frac{1}{P} (M - P \cdot 2x) = \frac{M - 2 P x}{P}
$$

Set the derivative equal to zero:

$$
\frac{M - 2 P x}{P} = 0 \quad \Rightarrow \quad M - 2 P x = 0 \quad \Rightarrow \quad x = \frac{M}{2 P}
$$

Check the second derivative to confirm a maximum:

$$
f''(x) = \frac{1}{P} (-2 P) = -2 < 0
$$

Since $f''(x) < 0$  , $x = \frac{M}{2 P}$  is a maximum.

#### Find y∗ y^\*

Substitute $x^* = \frac{M}{2 P}$  into the budget constraint:

$$
P \cdot \frac{M}{2 P} + P y^* = M
$$
 
$$
\frac{M}{2} + P y^* = M
$$
 
$$
P y^* = M - \frac{M}{2} = \frac{M}{2}
$$
 
$$
y^* = \frac{M}{2 P}
$$

So:

$$
x^* = \frac{M}{2 P}, \quad y^* = \frac{M}{2 P}
$$

Thus:

$$
x^* = y^*
$$

### Step 4: Verify with Marginal Utilities

To confirm, use the condition for utility maximization: the marginal utility per dollar spent should be equal for both goods. Since $P_X = P_Y = P$  :

$$
\frac{\partial u / \partial x}{P} = \frac{\partial u / \partial y}{P}
$$
 
$$
\frac{\partial u}{\partial x} = \frac{\partial u}{\partial y}
$$

Compute the partial derivatives:

$$
u(x, y) = A (xy)^{1/2}
$$
 
$$
\frac{\partial u}{\partial x} = A \cdot \frac{1}{2} (xy)^{-1/2} \cdot y = \frac{A y}{2 \sqrt{xy}}
$$
 
$$
\frac{\partial u}{\partial y} = A \cdot \frac{1}{2} (xy)^{-1/2} \cdot x = \frac{A x}{2 \sqrt{xy}}
$$

Set them equal:

$$
\frac{A y}{2 \sqrt{xy}} = \frac{A x}{2 \sqrt{xy}}
$$

Since $\sqrt{xy} \neq 0$  (assuming $x, y > 0$  ) and $A > 0$  :

$$
y = x
$$

This condition, along with the budget constraint, confirms $x^* = y^* = \frac{M}{2 P}$  .

### Step 5: Check Corner Solutions

If $x = 0$  :

$$
P \cdot 0 + P y = M \quad \Rightarrow \quad y = \frac{M}{P}
$$
 
$$
u(0, \frac{M}{P}) = A \sqrt{0 \cdot \frac{M}{P}} = 0
$$

If $y = 0$  :

$$
u(\frac{M}{P}, 0) = 0
$$

Compare with the interior solution:

$$
u\left(\frac{M}{2 P}, \frac{M}{2 P}\right) = A \sqrt{\frac{M}{2 P} \cdot \frac{M}{2 P}} = A \sqrt{\frac{M^2}{4 P^2}} = A \cdot \frac{M}{2 P} > 0
$$

Since $M > 0$  , $P > 0$  , the interior solution yields positive utility, while corner solutions yield zero, confirming the interior solution is the maximum.

### Step 6: Evaluate the Options

- **(A) $x^* > y^*$** : False, since $x^* = y^*$  .
- **(B) $x^* = y^*$** : True, as derived.
- **(C) $x^* < y^*$** : False, since $x^* = y^*$  .
- **(D) $x^* + y^* = M$** :
	$$
	x^* + y^* = \frac{M}{2 P} + \frac{M}{2 P} = \frac{M}{P}
	$$
	 Since $P > 1$  , $\frac{M}{P} < M$  , so $x^* + y^* \neq M$  , making (D) false.

### Final Answer

The statement that must always be true is:

$$
\text{(B) it must always be that } x^* = y^*
$$

what are the general steps i should take as fella from the fucking streets to go through these sort of questions that appear in the above pdf [admission.isical.ac.in](https://admission.isical.ac.in/Programs/MSQE.html)

No response.

Interrupted what are the general steps i should take as fella from the fucking streets to go through these sort of questions that appear in the above website that have attached with [admission.isical.ac.in](https://admission.isical.ac.in/Programs/MSQE.html)

No response. https://grok.com/chat/5ed2d142-4d00-49a0-9b5e-6cfd0247a8dc