---
title: "Integer Solutions to \xy - 6x + y = 0\ - Grok"
source: "https://grok.com/chat/3976c0ab-a904-4901-b7a8-f364acb250fb"
author:
published:
created: 2025-04-09
description: "Grok is a free AI assistant designed by xAI to maximize truth and objectivity. Grok offers real-time search, image generation, trend analysis, and more."
tags:
  - "clippings"
---
Refer to the following content:image.png

To determine the number of integer solutions $(x, y)$ to the equation $xy - 6(x + y) = 0$ with the condition $x \leq y$ , we need to find all pairs of integers (positive, negative, or zero) that satisfy both the equation and the constraint. Let’s solve this step-by-step.

### Step 1: Simplify the Equation

Start with the given equation:

$xy - 6(x + y) = 0$

Expand and rearrange it:

$xy - 6x - 6y = 0$

This form suggests a possible factorization. To make it more manageable, consider completing an expression. Notice that:

$xy - 6x - 6y + 36 = (x - 6)(y - 6)$

So:

$xy - 6x - 6y = (x - 6)(y - 6) - 36$

Since the original equation equals zero:

$(x - 6)(y - 6) - 36 = 0$

$(x - 6)(y - 6) = 36$

This is a key simplification. Now, we need to find integer pairs $(x, y)$ such that the product $(x - 6)(y - 6) = 36$ , and $x \leq y$ .

### Step 2: Define Variables

Let:

- $a = x - 6$
- $b = y - 6$

Then the equation becomes:

$a \cdot b = 36$

And:

- $x = a + 6$
- $y = b + 6$

The condition $x \leq y$ translates to:

$a + 6 \leq b + 6$

$a \leq b$

Since $x$ and $y$ are integers, $a$ and $b$ are also integers. Our task is to find all integer pairs $(a, b)$ such that $a \cdot b = 36$ and $a \leq b$ , then compute the corresponding $(x, y)$ pairs.

### Step 3: Find Integer Pairs (a,b)(a, b)

Since $a$ and $b$ are integers whose product is 36 (a positive number), they must both be positive or both be negative. We’ll consider both cases and list all pairs where $a \leq b$ .

#### Case 1: Both aa and bb are Positive

List the positive divisors of 36: 1, 2, 3, 4, 6, 9, 12, 18, 36. For each divisor $a$ , compute $b = \frac{36}{a}$ , and keep pairs where $a \leq b$ :

- $a = 1$  , $b = \frac{36}{1} = 36$  , $1 \leq 36$
- $a = 2$  , $b = \frac{36}{2} = 18$  , $2 \leq 18$
- $a = 3$  , $b = \frac{36}{3} = 12$  , $3 \leq 12$
- $a = 4$  , $b = \frac{36}{4} = 9$  , $4 \leq 9$
- $a = 6$  , $b = \frac{36}{6} = 6$  , $6 \leq 6$
- $a = 9$  , $b = \frac{36}{9} = 4$  , $9 > 4$  (discard)
- $a = 12$  , $b = \frac{36}{12} = 3$  , $12 > 3$  (discard)
- $a = 18$  , $b = \frac{36}{18} = 2$  , $18 > 2$  (discard)
- $a = 36$  , $b = \frac{36}{36} = 1$  , $36 > 1$  (discard)

So, the valid pairs are:

1. $(1, 36)$
2. $(2, 18)$
3. $(3, 12)$
4. $(4, 9)$
5. $(6, 6)$

#### Case 2: Both aa and bb are Negative

List the negative divisors of 36: -1, -2, -3, -4, -6, -9, -12, -18, -36. For each $a$ , compute $b = \frac{36}{a}$ , and keep pairs where $a \leq b$ (noting that for negative numbers, $a \leq b$ means $a$ is more negative or equal to $b$ ):

- $a = -1$  , $b = \frac{36}{-1} = -36$  , $-1 > -36$  (discard)
- $a = -2$  , $b = \frac{36}{-2} = -18$  , $-2 > -18$  (discard)
- $a = -3$  , $b = \frac{36}{-3} = -12$  , $-3 > -12$  (discard)
- $a = -4$  , $b = \frac{36}{-4} = -9$  , $-4 > -9$  (discard)
- $a = -6$  , $b = \frac{36}{-6} = -6$  , $-6 \leq -6$
- $a = -9$  , $b = \frac{36}{-9} = -4$  , $-9 < -4$
- $a = -12$  , $b = \frac{36}{-12} = -3$  , $-12 < -3$
- $a = -18$  , $b = \frac{36}{-18} = -2$  , $-18 < -2$
- $a = -36$  , $b = \frac{36}{-36} = -1$  , $-36 < -1$

Valid pairs are:

1. $(-6, -6)$
2. $(-9, -4)$
3. $(-12, -3)$
4. $(-18, -2)$
5. $(-36, -1)$

### Step 4: Compute Corresponding (x,y)(x, y) Pairs

For each pair $(a, b)$ , compute $x = a + 6$ , $y = b + 6$ .

**Positive Pairs:**

1. $(1, 36)$  : $x = 1 + 6 = 7$  , $y = 36 + 6 = 42$  , pair: $(7, 42)$
2. $(2, 18)$  : $x = 2 + 6 = 8$  , $y = 18 + 6 = 24$  , pair: $(8, 24)$
3. $(3, 12)$  : $x = 3 + 6 = 9$  , $y = 12 + 6 = 18$  , pair: $(9, 18)$
4. $(4, 9)$  : $x = 4 + 6 = 10$  , $y = 9 + 6 = 15$  , pair: $(10, 15)$
5. $(6, 6)$  : $x = 6 + 6 = 12$  , $y = 6 + 6 = 12$  , pair: $(12, 12)$

**Negative Pairs:**

1. $(-6, -6)$  : $x = -6 + 6 = 0$  , $y = -6 + 6 = 0$  , pair: $(0, 0)$
2. $(-9, -4)$  : $x = -9 + 6 = -3$  , $y = -4 + 6 = 2$  , pair: $(-3, 2)$
3. $(-12, -3)$  : $x = -12 + 6 = -6$  , $y = -3 + 6 = 3$  , pair: $(-6, 3)$
4. $(-18, -2)$  : $x = -18 + 6 = -12$  , $y = -2 + 6 = 4$  , pair: $(-12, 4)$
5. $(-36, -1)$  : $x = -36 + 6 = -30$  , $y = -1 + 6 = 5$  , pair: $(-30, 5)$

### Step 5: Verify Solutions

Check that each pair satisfies the original equation and the condition:

- $(7, 42)$  : $7 \cdot 42 - 6(7 + 42) = 294 - 6 \cdot 49 = 294 - 294 = 0$  , $7 \leq 42$
- $(8, 24)$  : $8 \cdot 24 - 6(8 + 24) = 192 - 6 \cdot 32 = 192 - 192 = 0$  , $8 \leq 24$
- $(9, 18)$  : $9 \cdot 18 - 6(9 + 18) = 162 - 6 \cdot 27 = 162 - 162 = 0$  , $9 \leq 18$
- $(10, 15)$  : $10 \cdot 15 - 6(10 + 15) = 150 - 6 \cdot 25 = 150 - 150 = 0$  , $10 \leq 15$
- $(12, 12)$  : $12 \cdot 12 - 6(12 + 12) = 144 - 6 \cdot 24 = 144 - 144 = 0$  , $12 \leq 12$
- $(0, 0)$  : $0 \cdot 0 - 6(0 + 0) = 0 - 0 = 0$  , $0 \leq 0$
- $(-3, 2)$  : $(-3) \cdot 2 - 6(-3 + 2) = -6 - 6(-1) = -6 + 6 = 0$  , $-3 \leq 2$
- $(-6, 3)$  : $(-6) \cdot 3 - 6(-6 + 3) = -18 - 6(-3) = -18 + 18 = 0$  , $-6 \leq 3$
- $(-12, 4)$  : $(-12) \cdot 4 - 6(-12 + 4) = -48 - 6(-8) = -48 + 48 = 0$  , $-12 \leq 4$
- $(-30, 5)$  : $(-30) \cdot 5 - 6(-30 + 5) = -150 - 6(-25) = -150 + 150 = 0$  , $-30 \leq 5$

All pairs satisfy both the equation and $x \leq y$ .

### Step 6: Count and Check for Completeness

We have 10 pairs:

1. $(7, 42)$
2. $(8, 24)$
3. $(9, 18)$
4. $(10, 15)$
5. $(12, 12)$
6. $(0, 0)$
7. $(-3, 2)$
8. $(-6, 3)$
9. $(-12, 4)$
10. $(-30, 5)$

All pairs are distinct. Since 36 has 18 divisors (9 positive, 9 negative), there are 18 possible $(a, b)$ pairs, but only 10 satisfy $a \leq b$ , corresponding to 10 $(x, y)$ pairs where $x \leq y$ . Pairs where $a > b$ (e.g., $(36, 1) \rightarrow (42, 7)$ ) have $x > y$ and are excluded.

### Final Answer

The number of integer solutions is 10, matching option (B).

**Answer: 10**

How could I have arrived at this method because i was running in circles. Moving the expressions around but this did not strike me, what thought process and what to keep in mind so this comes naturally?

To address your query about how to arrive at the method for solving the equation $xy - 6(x + y) = 0$ for integer solutions with $x \leq y$ , and to avoid running in circles, let’s break down the thought process that leads to the effective approach. I’ll explain how you can develop this intuition naturally and what to keep in mind for similar problems.

### Step 1: Recognize the Goal and Simplify the Equation

When faced with an equation like $xy - 6(x + y) = 0$ , the goal is to find all integer pairs $(x, y)$ that satisfy it, with the constraint $x \leq y$ . The equation involves a product term $xy$ and linear terms $-6x$ and $-6y$ , suggesting that manipulation might reveal a pattern or factorization. Instead of moving terms around aimlessly, start by aiming to transform the equation into a form that’s easier to analyze for integer solutions.

Let’s rewrite the equation:

$xy - 6x - 6y = 0$

This doesn’t immediately factor, and adding or subtracting terms randomly might feel like spinning in circles. A key insight is to look for a way to relate $xy - 6x - 6y$ to a recognizable form, such as a product or a completed expression. One effective technique for expressions like this—where you have a product and subtracted terms—is to try completing a pattern, similar to completing the square in quadratic equations.

### Step 2: Experiment with Factorization by Adding a Constant

Notice the coefficients: $-6x$ and $-6y$ suggest that the number 6 might play a role in factoring. A useful trick is to add and subtract a constant to both sides to form a product. Let’s explore this by considering:

$xy - 6x - 6y + k = k$

We want the left side to factor nicely. Test the expression $(x - 6)(y - 6)$ :

$(x - 6)(y - 6) = xy - 6x - 6y + 36$

This is promising! Compare it to our equation:

$xy - 6x - 6y = (x - 6)(y - 6) - 36$

Since the original equation equals 0:

$xy - 6x - 6y = 0$

$(x - 6)(y - 6) - 36 = 0$

$(x - 6)(y - 6) = 36$

This transformation is the breakthrough! Instead of a mixed expression, we now have a single product equal to a constant, which is much easier to handle when seeking integer solutions.

**Why this works:** The terms $-6x$ and $-6y$ hint at subtracting 6 from $x$ and $y$ , and the constant 36 (which is $6 \cdot 6$ ) balances the equation. This isn’t random—it’s guided by recognizing that $xy - 6x - 6y + 36$ resembles a binomial expansion.

### Step 3: Solve Using Integer Pairs

Define:

- $a = x - 6$
- $b = y - 6$

Then:

$a \cdot b = 36$

And since $x = a + 6$ and $y = b + 6$ , the condition $x \leq y$ becomes:

$a + 6 \leq b + 6$

$a \leq b$

Now, find all integer pairs $(a, b)$ such that $a \cdot b = 36$ and $a \leq b$ . Since 36 is positive, $a$ and $b$ are either both positive or both negative.

#### Positive Pairs

List the positive factor pairs of 36 where the first number is less than or equal to the second:

- $1 \cdot 36 = 36$ , $1 \leq 36$
- $2 \cdot 18 = 36$ , $2 \leq 18$
- $3 \cdot 12 = 36$ , $3 \leq 12$
- $4 \cdot 9 = 36$ , $4 \leq 9$
- $6 \cdot 6 = 36$ , $6 \leq 6$

Pairs: $(1, 36)$ , $(2, 18)$ , $(3, 12)$ , $(4, 9)$ , $(6, 6)$ .

#### Negative Pairs

If both $a$ and $b$ are negative, let $a = -d$ , $b = -e$ , where $d$ and $e$ are positive, and:

$(-d) \cdot (-e) = de = 36$

Since $a \leq b$ :

$-d \leq -e$

$d \geq e$

List pairs where $d \cdot e = 36$ and $d \geq e$ :

- $36 \cdot 1 = 36$ , $36 \geq 1$
- $18 \cdot 2 = 36$ , $18 \geq 2$
- $12 \cdot 3 = 36$ , $12 \geq 3$
- $9 \cdot 4 = 36$ , $9 \geq 4$
- $6 \cdot 6 = 36$ , $6 \geq 6$

So, $(d, e) = (36, 1), (18, 2), (12, 3), (9, 4), (6, 6)$ , and:

- $a = -36$ , $b = -1$
- $a = -18$ , $b = -2$
- $a = -12$ , $b = -3$
- $a = -9$ , $b = -4$
- $a = -6$ , $b = -6$

Pairs: $(-36, -1)$ , $(-18, -2)$ , $(-12, -3)$ , $(-9, -4)$ , $(-6, -6)$ .

#### Compute (x,y)(x, y)

- Positive pairs:
	- $(1, 36) \rightarrow (7, 42)$
	- $(2, 18) \rightarrow (8, 24)$
	- $(3, 12) \rightarrow (9, 18)$
	- $(4, 9) \rightarrow (10, 15)$
	- $(6, 6) \rightarrow (12, 12)$
- Negative pairs:
	- $(-36, -1) \rightarrow (-30, 5)$
	- $(-18, -2) \rightarrow (-12, 4)$
	- $(-12, -3) \rightarrow (-6, 3)$
	- $(-9, -4) \rightarrow (-3, 2)$
	- $(-6, -6) \rightarrow (0, 0)$

Total: 10 pairs.

### Step 4: Verify Solutions

Each pair satisfies $xy - 6(x + y) = 0$ and $x \leq y$ (e.g., for $(7, 42)$ : $7 \cdot 42 - 6(7 + 42) = 294 - 294 = 0$ ), confirming the method’s correctness.

### How to Develop This Thought Process

1. **Look for Patterns:** When you see $xy - 6x - 6y$ , notice the repeated 6. This suggests a form like $(x - 6)(y - 6)$ . Train yourself to spot coefficients that might align with a product.
2. **Try Completion Techniques:** If direct factoring fails, add and subtract a constant (here, 36) to form a product. This mimics completing the square and is a standard algebraic strategy.
3. **Substitute Variables:** Defining $a = x - 6$ , $b = y - 6$ simplifies the equation. When stuck, shifting variables by a constant related to the coefficients can clarify the structure.
4. **Focus on Integers Early:** Since the problem asks for integer solutions, aim for a form (like $a \cdot b = 36$ ) where integer constraints are straightforward.
5. **Avoid Random Moves:** Instead of shuffling terms without direction, hypothesize a form (e.g., a product) and test it. Here, testing $(x - 6)(y - 6)$ was purposeful.
6. **Practice Similar Problems:** Solve equations like $xy - a(x + y) = b$ to build intuition for this pattern.

### What to Keep in Mind

- **Coefficient Clues:** Use numbers like 6 as hints for subtraction or addition in factors.
- **Goal-Oriented Manipulation:** Always work toward a form that leverages the problem’s constraints (integers, inequalities).
- **Systematic Pairing:** Once you reach $a \cdot b = 36$ , list pairs methodically, considering signs and conditions.

By focusing on these strategies, this approach will feel more natural over time, preventing the cycle of aimless manipulation. The key is purposeful transformation guided by the equation’s structure and the problem’s requirements.

is that all what are the approaches in these type of questions

To determine the number of integer solutions $(x, y)$ to the equation $xy - 6(x + y) = 0$ where $x \leq y$ , we need to systematically find all pairs of integers that satisfy both the equation and the given condition. Let’s solve this step-by-step and then explore the approaches typically used for such problems.

### Solving the Problem

Start with the given equation:

$xy - 6(x + y) = 0$

Simplify by expanding and rearranging:

$xy - 6x - 6y = 0$

To make this easier to factor, add 36 to both sides (a technique to complete a pattern):

$xy - 6x - 6y + 36 = 36$

The left-hand side now resembles a factored form:

$(x - 6)(y - 6) = 36$

This transformation is key. Define:

- $a = x - 6$
- $b = y - 6$

Then the equation becomes:

$a b = 36$

Since $x = a + 6$  and $y = b + 6$  , the condition $x \leq y$  translates to:

$a + 6 \leq b + 6$

$a \leq b$

We need to find all integer pairs $(a, b)$ such that $a b = 36$  and $a \leq b$  , then convert them back to $(x, y)$ .

#### Finding Integer Pairs (a,b)(a, b)

Since $a b = 36$  and 36 is positive, $a$  and $b$  must both be positive or both negative (if one were positive and the other negative, the product would be negative).

**Positive Pairs:**

List the positive factor pairs of 36 where $a \leq b$  :

- $1 \times 36 = 36$  : $(1, 36)$
- $2 \times 18 = 36$  : $(2, 18)$
- $3 \times 12 = 36$  : $(3, 12)$
- $4 \times 9 = 36$  : $(4, 9)$
- $6 \times 6 = 36$  : $(6, 6)$

Pairs like $(9, 4)$ have $9 > 4$  , so they’re excluded. There are 5 pairs: $(1, 36)$ , $(2, 18)$ , $(3, 12)$ , $(4, 9)$ , $(6, 6)$ .

**Negative Pairs:**

For both $a$  and $b$  negative, consider $a = -d$  , $b = -e$  , where $d$  and $e$  are positive integers and $(-d)(-e) = de = 36$  . The condition $a \leq b$  becomes $-d \leq -e$  , or $d \geq e$  . List pairs where $de = 36$  and $d \geq e$  :

- $36 \times 1 = 36$  : $d = 36$  , $e = 1$  , so $a = -36$  , $b = -1$
- $18 \times 2 = 36$  : $d = 18$  , $e = 2$  , so $a = -18$  , $b = -2$
- $12 \times 3 = 36$  : $d = 12$  , $e = 3$  , so $a = -12$  , $b = -3$
- $9 \times 4 = 36$  : $d = 9$  , $e = 4$  , so $a = -9$  , $b = -4$
- $6 \times 6 = 36$  : $d = 6$  , $e = 6$  , so $a = -6$  , $b = -6$

Thus, the pairs are: $(-36, -1)$ , $(-18, -2)$ , $(-12, -3)$ , $(-9, -4)$ , $(-6, -6)$ —also 5 pairs.

**Total Pairs:**

- Positive: $(1, 36)$ , $(2, 18)$ , $(3, 12)$ , $(4, 9)$ , $(6, 6)$
- Negative: $(-36, -1)$ , $(-18, -2)$ , $(-12, -3)$ , $(-9, -4)$ , $(-6, -6)$

Total of 10 pairs.

#### Converting to (x,y)(x, y)

Compute $x = a + 6$  , $y = b + 6$  :

- $(1, 36)$ : $x = 1 + 6 = 7$  , $y = 36 + 6 = 42$  → $(7, 42)$
- $(2, 18)$ : $x = 2 + 6 = 8$  , $y = 18 + 6 = 24$  → $(8, 24)$
- $(3, 12)$ : $x = 3 + 6 = 9$  , $y = 12 + 6 = 18$  → $(9, 18)$
- $(4, 9)$ : $x = 4 + 6 = 10$  , $y = 9 + 6 = 15$  → $(10, 15)$
- $(6, 6)$ : $x = 6 + 6 = 12$  , $y = 6 + 6 = 12$  → $(12, 12)$
- $(-6, -6)$ : $x = -6 + 6 = 0$  , $y = -6 + 6 = 0$  → $(0, 0)$
- $(-9, -4)$ : $x = -9 + 6 = -3$  , $y = -4 + 6 = 2$  → $(-3, 2)$
- $(-12, -3)$ : $x = -12 + 6 = -6$  , $y = -3 + 6 = 3$  → $(-6, 3)$
- $(-18, -2)$ : $x = -18 + 6 = -12$  , $y = -2 + 6 = 4$  → $(-12, 4)$
- $(-36, -1)$ : $x = -36 + 6 = -30$  , $y = -1 + 6 = 5$  → $(-30, 5)$

**Verification:**

Check a few pairs:

- $(7, 42)$ : $7 \cdot 42 - 6(7 + 42) = 294 - 6 \cdot 49 = 294 - 294 = 0$
- $(0, 0)$ : $0 \cdot 0 - 6(0 + 0) = 0 - 0 = 0$
- $(-3, 2)$ : $(-3) \cdot 2 - 6(-3 + 2) = -6 - 6(-1) = -6 + 6 = 0$

All satisfy the equation, and $x \leq y$  holds (e.g., $7 \leq 42$  , $0 \leq 0$  , $-3 \leq 2$  ).

**Conclusion:**

There are 10 distinct integer solutions: $(7, 42)$ , $(8, 24)$ , $(9, 18)$ , $(10, 15)$ , $(12, 12)$ , $(0, 0)$ , $(-3, 2)$ , $(-6, 3)$ , $(-12, 4)$ , $(-30, 5)$ . Thus, the number of solutions is 10.

### Approaches to These Types of Questions

For equations involving integer solutions (Diophantine equations) with constraints like $x \leq y$  , several approaches are common:

1. **Algebraic Manipulation and Factoring:**
	- Transform the equation into a recognizable form, as we did by adding 36 to get $(x - 6)(y - 6) = 36$ . Introduce substitutions (e.g., $a = x - 6$  , $b = y - 6$  ) to simplify, then find factor pairs of the constant (36) under the constraint $a \leq b$  . This is efficient for equations resembling product forms.
2. **Solve for One Variable:**
	- Rewrite the equation as $xy - 6y = 6x$  , so $y(x - 6) = 6x$  . If $x \neq 6$  : $y = \frac{6x}{x - 6}$
	- $y$  must be an integer, so $x - 6$  must divide $6x$  . Set $d = x - 6$  , a divisor of 36, then $x = d + 6$  , $y = \frac{36}{d} + 6$  , and check $x \leq y$  (i.e., $d \leq \frac{36}{d}$  ). This confirms the same pairs but requires handling $x = 6$  separately ( $y = 12$  ).
3. **Factor Pair Enumeration:**
	- Directly list divisors of 36 (positive: 1, 2, 3, 4, 6, 9, 12, 18, 36; negative: -1, -2, -3, -4, -6, -9, -12, -18, -36)). For each $d$  , compute $x = d + 6$  , $y = \frac{36}{d} + 6$  , and select pairs where $x \leq y$  . This is systematic but requires filtering.
4. **Geometric or Symmetric Insight:**
	- Recognize that $(x - 6)(y - 6) = 36$ is a hyperbola in the $xy$  \-plane. Integer solutions are lattice points on this curve, and $x \leq y$  restricts us to one region. This is more visual but less practical here.
5. **Testing Values:**
	- Plug in integer $x$  and solve for $y$  , checking if $y$  is an integer and $x \leq y$  . This is brute-force and inefficient but viable for small constants.

The first approach (factoring) is most efficient here, leveraging the equation’s structure. The second (solving for $y$  ) provides a cross-check, ensuring all solutions are captured. For similar problems:

- **Linear Diophantine Equations:** Use modular arithmetic or the Euclidean algorithm.
- **Quadratic Forms:** Complete the square or use number theory (e.g., Pell equations).
- **Constraints:** Adjust pair selection (e.g., $x \geq 0$  changes the count).

For this problem, the answer is 10 integer solutions. https://grok.com/chat/3976c0ab-a904-4901-b7a8-f364acb250fb