---
title: "Slope of Inverse Demand Function - Grok"
source: "https://grok.com/chat/9d0949ff-6cb9-4434-9d8f-a8d73da47f52"
author:
published:
created: 2025-04-03
description: "Grok is a free AI assistant designed by xAI to maximize truth and objectivity. Grok offers real-time search, image generation, trend analysis, and more."
tags:
  - "clippings"
---
Refer to the following content:image.png

To determine the slope of the inverse demand function $p(q)$  in the given microeconomic scenario, let’s carefully derive the solution step by step based on the problem’s setup.

We are dealing with a unit mass of consumers, each of whom decides to buy either one unit of a product or nothing, depending on their valuation $\theta$  . The valuation $\theta$  is distributed over the interval $[\underline{\theta}, \overline{\theta}]$  according to a cumulative distribution function (CDF) $F(\theta)$  , where $F(\theta)$  represents the proportion of consumers with a valuation less than or equal to $\theta$  . Assuming $F(\theta)$  is differentiable, its derivative $F'(\theta)$  is the probability density function (PDF).

### Step 1: Define Consumer Behavior and Demand

Each consumer purchases one unit if the price $p$  is less than or equal to their valuation $\theta$  (i.e., $p \leq \theta$  ), as this implies their utility from buying, $\theta - p$  , is non-negative, while their utility from not buying is zero. For a given price $p$  , the proportion of consumers with $\theta \geq p$  —those who will buy—is $1 - F(p)$  , since $F(p) = \text{Prob}(\theta \leq p)$  and thus $1 - F(p) = \text{Prob}(\theta > p)$  (assuming no mass points for simplicity). Given a unit mass of consumers, the aggregate demand $q$  at price $p$  is the total number of buyers, so:

$$
q = 1 - F(p)
$$

This is the demand function $q(p)$  .

### Step 2: Derive the Inverse Demand Function

The query asks for the inverse demand function $p(q)$  , which gives the price required to achieve a specific quantity demanded $q$  . Starting from the demand function:

$$
q = 1 - F(p)
$$

Solve for $p$  in terms of $q$  :

$$
F(p) = 1 - q
$$

Assuming $F$  is strictly increasing and continuous (so it has an inverse), apply the inverse function $F^{-1}$  :

$$
p = F^{-1}(1 - q)
$$

Thus, the inverse demand function is:

$$
p(q) = F^{-1}(1 - q)
$$

### Step 3: Compute the Slope of the Inverse Demand Function

We need the slope $p'(q)$  , the derivative of $p(q)$  with respect to $q$  . Using the chain rule, let’s differentiate $p(q) = F^{-1}(1 - q)$  . Define $u = 1 - q$  , so $p(q) = F^{-1}(u)$  , and:

$$
\frac{dp}{dq} = \frac{d}{dq} [F^{-1}(u)] = \frac{d}{du} [F^{-1}(u)] \cdot \frac{du}{dq}
$$
- Since $u = 1 - q$  , we have $\frac{du}{dq} = -1$  .
- For the derivative of the inverse function, if $g(u) = F^{-1}(u)$  , then $F(g(u)) = u$  . Differentiating both sides with respect to $u$  :
$$
F'(g(u)) \cdot g'(u) = 1 \implies g'(u) = \frac{1}{F'(g(u))}
$$

Here, $g(u) = F^{-1}(u)$  , so $\frac{d}{du} [F^{-1}(u)] = \frac{1}{F'(F^{-1}(u))}$  . Substituting $u = 1 - q$  :

$$
\frac{d}{du} [F^{-1}(u)] = \frac{1}{F'(F^{-1}(1 - q))}
$$

Since $p(q) = F^{-1}(1 - q)$  , this becomes:

$$
\frac{d}{du} [F^{-1}(u)] = \frac{1}{F'(p(q))}
$$

Thus:

$$
p'(q) = \frac{d}{du} [F^{-1}(u)] \cdot \frac{du}{dq} = \frac{1}{F'(p(q))} \cdot (-1) = -\frac{1}{F'(p(q))}
$$

### Step 4: Alternative Derivation via Implicit Differentiation

To confirm, use implicit differentiation on $q = 1 - F(p(q))$  :

$$
\frac{d}{dq} [q] = \frac{d}{dq} [1 - F(p(q))]
$$
- Left side: $1$
- Right side: $0 - F'(p(q)) \cdot p'(q)$  , since $\frac{d}{dq} [F(p(q))] = F'(p(q)) \cdot p'(q)$

So:

$$
1 = -F'(p(q)) \cdot p'(q)
$$
 
$$
p'(q) = -\frac{1}{F'(p(q))}
$$

Both methods agree, reinforcing confidence in the result.

### Step 5: Verify with Examples

- **Uniform Distribution**: If $F(\theta) = \theta$  on $[0, 1]$  , then $q = 1 - p$  , so $p = 1 - q$  , and $p'(q) = -1$  . Also, $F'(\theta) = 1$  , so $F'(p(q)) = 1$  , and $-\frac{1}{F'(p(q))} = -1$  , which matches.
- **Non-Uniform**: If $F(\theta) = \theta^2$  on $[0, 1]$  , then $q = 1 - p^2$  , so $p = \sqrt{1 - q}$  , and $p'(q) = -\frac{1}{2 \sqrt{1 - q}}$  . Here, $F'(\theta) = 2\theta$  , so $F'(p(q)) = 2 \sqrt{1 - q}$  , and $-\frac{1}{F'(p(q))} = -\frac{1}{2 \sqrt{1 - q}}$  , which matches.

### Step 6: Match with Options

The options are:

- (a) $p'(q) = -\frac{1}{F'(p(q))}$
- (b) $p'(q) = -F'(p(q))$
- (c) $p'(q) = -\frac{1}{F'(q)}$
- (d) $p'(q) = -F'(q)$

Our derivation gives $p'(q) = -\frac{1}{F'(p(q))}$  , matching option (a). Options (c) and (d) use $F'(q)$  , which is incorrect since $F'$  is defined over valuations $\theta$  , not quantities $q$  . Option (b) lacks the reciprocal, failing the non-uniform example (e.g., $-F'(p(0)) = -2 \neq -\frac{1}{2}$  ).

### Final Answer

The slope of the inverse demand function is:

$$
p'(q) = -\frac{1}{F'(p(q))}
$$

Thus, the correct answer is option (a).

how

It seems like your query might be incomplete, but based on the context provided, I’ll assume you’re asking, "How do you find the slope of the inverse demand function in this microeconomics problem?" Here’s a clear and complete explanation of how to do that.

---

### Problem Setup

In this microeconomics scenario, we have a unit mass of consumers, each deciding whether to buy one unit of a product or nothing, depending on their valuation $\theta$  . The valuation $\theta$  is distributed over an interval $[\underline{\theta}, \overline{\theta}]$  with a cumulative distribution function (CDF) $F(\theta)$  , which is differentiable, meaning it has a density function $f(\theta) = F'(\theta)$  . A consumer buys the product if the price $p$  is less than or equal to their valuation $\theta$  , because their utility $\theta - p \geq 0$  in that case. If $p > \theta$  , they don’t buy since their utility would be negative.

For a given price $p$  , the proportion of consumers with $\theta \geq p$  is $1 - F(p)$  , because $F(p)$  is the proportion with $\theta \leq p$  . Since there’s a unit mass of consumers, the total quantity demanded $q$  at price $p$  is:

$q = 1 - F(p)$

This is the demand function $q(p)$  . However, we need the **inverse demand function** $p(q)$  , which expresses the price as a function of quantity demanded, and then we need to find its slope, $p'(q)$  , the derivative of $p$  with respect to $q$  .

---

### Step 1: Derive the Inverse Demand Function

Start with the demand function:

$q = 1 - F(p)$

To find the inverse demand function, solve for $p$  in terms of $q$  :

$q = 1 - F(p)$

$F(p) = 1 - q$

Since $F(\theta)$  is a CDF and differentiable (with a positive density $F'(\theta) > 0$  ), it is strictly increasing and thus has an inverse, denoted $F^{-1}$  . Applying the inverse function:

$p = F^{-1}(1 - q)$

So, the inverse demand function is:

$p(q) = F^{-1}(1 - q)$

This gives the price $p$  that corresponds to a quantity demanded $q$  .

---

### Step 2: Find the Slope of the Inverse Demand Function

To find the slope, compute the derivative $p'(q) = \frac{dp}{dq}$  . Since $p(q) = F^{-1}(1 - q)$  , this involves differentiating an inverse function. Let’s use the chain rule by introducing a substitution.

Define:

$u = 1 - q$

Then:

$p = F^{-1}(u)$

Now, compute $\frac{dp}{dq}$  using the chain rule:

$\frac{dp}{dq} = \frac{dp}{du} \cdot \frac{du}{dq}$

- **Compute $\frac{du}{dq}$** :

$u = 1 - q$

$\frac{du}{dq} = \frac{d}{dq}(1 - q) = -1$

- **Compute $\frac{dp}{du}$** :

Since $p = F^{-1}(u)$  , we have $u = F(p)$  . Differentiate both sides of $u = F(p)$  with respect to $u$  :

$1 = F'(p) \cdot \frac{dp}{du}$

$\frac{dp}{du} = \frac{1}{F'(p)}$

Here, $F'(p) = f(p)$  is the density function evaluated at $p$  , and since $p = F^{-1}(u)$  , we can write this in terms of $q$  . Since $u = 1 - q$  , we have $p = F^{-1}(1 - q) = p(q)$  , so:

$\frac{dp}{du} = \frac{1}{F'(p(q))}$

- **Combine using the chain rule**:

$\frac{dp}{dq} = \frac{dp}{du} \cdot \frac{du}{dq} = \left( \frac{1}{F'(p(q))} \right) \cdot (-1)$

$p'(q) = -\frac{1}{F'(p(q))}$

This is the slope of the inverse demand function.

---

### Step 3: Verify with Implicit Differentiation

To confirm, use implicit differentiation on the original equation:

$q = 1 - F(p(q))$

Differentiate both sides with respect to $q$  :

- Left side:

$\frac{dq}{dq} = 1$

- Right side (using the chain rule):

$\frac{d}{dq} [1 - F(p(q))] = 0 - F'(p(q)) \cdot p'(q) = -F'(p(q)) \cdot p'(q)$

Equate both sides:

$1 = -F'(p(q)) \cdot p'(q)$

Solve for $p'(q)$  :

$p'(q) = \frac{1}{-F'(p(q))} = -\frac{1}{F'(p(q))}$

This matches our previous result, confirming the slope is:

$p'(q) = -\frac{1}{F'(p(q))}$

---

### Step 4: Economic Intuition

Economically, this makes sense. The term $F'(p(q)) = f(p(q))$  is the density of consumers with valuation $\theta = p(q)$  . If $F'(p(q))$  is large (high density), many consumers have valuations near $p(q)$  , so a small price decrease increases quantity demanded significantly, making the inverse demand curve flatter (less negative slope). If $F'(p(q))$  is small (low density), a larger price drop is needed to increase quantity, making the slope steeper (more negative). The expression $p'(q) = -\frac{1}{F'(p(q))}$  captures this inverse relationship.

---

### Step 5: Example Check

Consider a uniform distribution on $[0, 1]$  , where $F(\theta) = \theta$  :

- Demand: $q = 1 - F(p) = 1 - p$
- Inverse demand: $p = 1 - q$  , so $p(q) = 1 - q$
- Slope: $p'(q) = -1$
- Check: $F'(\theta) = 1$  , so $F'(p(q)) = F'(1 - q) = 1$  , and $-\frac{1}{F'(p(q))} = -\frac{1}{1} = -1$  , which matches.

For a non-uniform case, say $F(\theta) = \theta^2$  on $[0, 1]$  :

- $q = 1 - F(p) = 1 - p^2$
- $p^2 = 1 - q$  , $p = \sqrt{1 - q}$  (since $p \geq 0$  )
- $p(q) = (1 - q)^{1/2}$  , $p'(q) = \frac{1}{2} (1 - q)^{-1/2} \cdot (-1) = -\frac{1}{2 \sqrt{1 - q}}$
- $F'(\theta) = 2\theta$  , so $F'(p(q)) = 2 \sqrt{1 - q}$  , and $-\frac{1}{F'(p(q))} = -\frac{1}{2 \sqrt{1 - q}}$  , which matches.

Both examples confirm the result.

---

### Final Result

The slope of the inverse demand function is:

$p'(q) = -\frac{1}{F'(p(q))}$

This is how you find it: derive the inverse demand $p(q) = F^{-1}(1 - q)$  from $q = 1 - F(p)$  , then differentiate using the chain rule or implicit differentiation, yielding the slope in terms of the density $F'$  evaluated at $p(q)$  .

I did not understand the derivation of the demand function can you explain more clearly

Let’s derive the demand function step by step in a clear and straightforward way. The goal is to understand how we arrive at the total quantity demanded, $q(p)$  , as a function of price $p$  , given the setup of the problem.

### Step 1: Understand the Setup

Imagine there’s a group of consumers, and their total “amount” is normalized to 1 (this is what “unit mass” means—it’s a simplification so we can work with proportions). Each consumer has a valuation $\theta$  , which is how much they’re willing to pay for one unit of a product. These valuations vary across consumers and are distributed over some range, say from a minimum $\underline{\theta}$  to a maximum $\overline{\theta}$  . This distribution is described by a cumulative distribution function (CDF) $F(\theta)$  , where:

- $F(\theta)$  is the proportion of consumers with a valuation less than or equal to $\theta$  .
- Since it’s a CDF, $F(\underline{\theta}) = 0$  (no one has a valuation below the minimum), and $F(\overline{\theta}) = 1$  (everyone has a valuation at or below the maximum).

### Step 2: Consumer Behavior

Each consumer decides whether to buy one unit of the product based on its price $p$  :

- **If $p \leq \theta$** : The consumer’s valuation is at least as high as the price, so they buy 1 unit. Their utility (benefit) is $\theta - p \geq 0$  , which is non-negative, making the purchase worthwhile.
- **If $p > \theta$** : The price exceeds their valuation, so they don’t buy (they’d get negative utility, $\theta - p < 0$  ).

So, at a given price $p$  , only consumers with $\theta \geq p$  will buy.

### Step 3: Find the Proportion of Buyers

We need to determine what fraction of consumers have a valuation $\theta \geq p$  , because these are the ones who will buy:

- $F(p)$  is the proportion of consumers with $\theta \leq p$  .
- Since the total proportion of consumers is 1 (unit mass), the proportion with $\theta > p$  is $1 - F(p)$  .
- The condition for buying is $p \leq \theta$  , or equivalently $\theta \geq p$  . In math terms, the proportion of consumers with $\theta \geq p$  is the probability $P(\theta \geq p)$  .

For a continuous distribution (where there’s no “jump” or mass of consumers at exactly $\theta = p$  ), the probability of $\theta$  being exactly equal to $p$  is zero. So, $P(\theta \geq p) = P(\theta > p) = 1 - F(p)$  . This means the proportion of consumers who buy—those with $\theta \geq p$  —is simply:

$1 - F(p)$

### Step 4: Calculate Total Quantity Demanded

Since there’s a unit mass of consumers (total “number” = 1), and each buyer purchases exactly 1 unit, the total quantity demanded $q$  at price $p$  is equal to the proportion of consumers who buy:

$q(p) = 1 - F(p)$

This is the demand function! It tells us how much of the product is demanded at any price $p$  .

### Step 5: Check the Logic

Let’s test this with extreme cases to ensure it makes sense:

- **If $p > \overline{\theta}$** : The price is higher than the highest valuation. Then, $F(p) = 1$  (since all $\theta \leq \overline{\theta} < p$  ), so: $q(p) = 1 - F(p) = 1 - 1 = 0$  No one buys, which is correct.
- **If $p < \underline{\theta}$** : The price is below the lowest valuation. Then, $F(p) = 0$  (since no $\theta$  is less than $\underline{\theta}$  ), so: $q(p) = 1 - F(p) = 1 - 0 = 1$  Everyone buys, which makes sense.
- **If $\underline{\theta} < p < \overline{\theta}$** : $F(p)$  is between 0 and 1, so $q(p) = 1 - F(p)$  is between 0 and 1, representing some fraction of consumers buying. This aligns with having a mix of buyers and non-buyers.

### Alternative Perspective: Using the Density Function

If $F(\theta)$  is differentiable, it has a density function $f(\theta) = F'(\theta)$  , which describes the “spread” of valuations. The proportion of consumers with $\theta \geq p$  can also be found by integrating the density from $p$  to $\overline{\theta}$  :

$P(\theta \geq p) = \int_p^{\overline{\theta}} f(\theta) \, d\theta$

Since $F(\theta)$  is the integral of $f(\theta)$  from $\underline{\theta}$  to $\theta$  , we have:

$\int_p^{\overline{\theta}} f(\theta) \, d\theta = F(\overline{\theta}) - F(p)$

And because $F(\overline{\theta}) = 1$  :

$F(\overline{\theta}) - F(p) = 1 - F(p)$

This matches our result: $q(p) = 1 - F(p)$  . So, whether we use the CDF directly or the density, we get the same demand function.

### Final Answer

The demand function is:

$q(p) = 1 - F(p)$

This represents the total quantity demanded at price $p$  , based on the proportion of consumers whose valuations are at least $p$  , given a unit mass of consumers distributed according to $F(\theta)$  . I hope this step-by-step explanation makes the derivation clear!

Solve the question in the image again for clarity and explain everything in detail

Let’s dive into finding the slope of the inverse demand function in a microeconomic context with a clear, step-by-step approach. We’re dealing with a unit mass of consumers, meaning the total “number” of consumers is normalized to 1 for simplicity. Each consumer has a valuation $\theta$  for a product, distributed over an interval $[\underline{\theta}, \overline{\theta}]$  according to a cumulative distribution function (CDF) $F(\theta)$  , which is differentiable. A consumer buys one unit of the product if the price $p$  is less than or equal to their valuation $\theta$  ; otherwise, they don’t buy. Our goal is to determine the slope of the inverse demand function $p(q)$  , where $q$  is the quantity demanded, and identify the correct expression from the options provided.

---

### Step 1: Define the Demand Function q(p) q(p)

First, let’s establish the demand function $q(p)$  , which tells us the quantity demanded at a given price $p$  . Since there’s a unit mass of consumers (total “number” = 1), the quantity demanded is the proportion of consumers willing to buy at price $p$  . A consumer buys if their valuation $\theta \geq p$  . Given $F(\theta)$  is the CDF, $F(p)$  represents the proportion of consumers with $\theta \leq p$  . Thus, the proportion with $\theta > p$  is $1 - F(p)$  .

Because $F(\theta)$  is differentiable, it has a density $f(\theta) = F'(\theta)$  , and since $\theta$  is continuous, the probability that $\theta = p$  is zero. Therefore, the proportion of consumers with $\theta \geq p$  is also $1 - F(p)$  . This proportion is the quantity demanded:

$$
q(p) = 1 - F(p)
$$

This makes sense: as price $p$  increases, $F(p)$  increases (since $F$  is non-decreasing), and $q(p)$  decreases, reflecting typical demand behavior.

---

### Step 2: Derive the Inverse Demand Function p(q) p(q)

The inverse demand function $p(q)$  gives the price as a function of quantity. To find it, we start with the demand function:

$$
q = 1 - F(p)
$$

Solve for $p$  in terms of $q$  :

$$
F(p) = 1 - q
$$

Assuming $F$  is strictly increasing (implied by differentiability and a positive density $f(\theta) > 0$  ), $F$  has an inverse $F^{-1}$  . Apply $F^{-1}$  to both sides:

$$
p = F^{-1}(1 - q)
$$

So, the inverse demand function is:

$$
p(q) = F^{-1}(1 - q)
$$

This expresses the price that corresponds to a given quantity demanded. When $q = 0$  , $p = F^{-1}(1) = \overline{\theta}$  (the highest valuation, since $F(\overline{\theta}) = 1$  ), and as $q$  approaches 1, $1 - q \to 0$  , so $p \to F^{-1}(0) = \underline{\theta}$  , aligning with the valuation bounds.

---

### Step 3: Compute the Slope of the Inverse Demand Function

We need the slope, $p'(q) = \frac{dp}{dq}$  . Since $p(q) = F^{-1}(1 - q)$  , we’ll use the chain rule and the derivative of an inverse function. Define:

$$
u = 1 - q
$$

Then:

$$
p(q) = F^{-1}(u)
$$

Differentiate with respect to $q$  :

$$
\frac{dp}{dq} = \frac{d}{dq} [F^{-1}(u)] = \frac{d F^{-1}(u)}{du} \cdot \frac{du}{dq}
$$
- Compute $\frac{du}{dq}$  :
$$
u = 1 - q \quad \Rightarrow \quad \frac{du}{dq} = -1
$$
- Compute $\frac{d F^{-1}(u)}{du}$  : If $y = F^{-1}(u)$  , then $F(y) = u$  . Differentiate both sides with respect to $u$  :
$$
F'(y) \cdot \frac{dy}{du} = 1
$$
 
$$
\frac{dy}{du} = \frac{1}{F'(y)} = \frac{1}{F'(F^{-1}(u))}
$$

Since $y = F^{-1}(u) = p(q)$  and $u = 1 - q$  , we have $p(q) = F^{-1}(1 - q)$  . Thus:

$$
\frac{d F^{-1}(u)}{du} = \frac{1}{F'(F^{-1}(u))} = \frac{1}{F'(p(q))}
$$

Combine:

$$
p'(q) = \frac{d F^{-1}(u)}{du} \cdot \frac{du}{dq} = \frac{1}{F'(p(q))} \cdot (-1) = -\frac{1}{F'(p(q))}
$$

So, the slope is:

$$
p'(q) = -\frac{1}{F'(p(q))}
$$

Here, $F'(p(q)) = f(p(q))$  , the probability density function at $p(q)$  , which is positive since $F$  is increasing.

---

### Step 4: Alternative Derivation for Confirmation

Let’s confirm using implicit differentiation. Start with:

$$
q = 1 - F(p(q))
$$

Differentiate both sides with respect to $q$  :

$$
1 = -\frac{d}{dq} [F(p(q))]
$$

Apply the chain rule:

$$
\frac{d}{dq} [F(p(q))] = F'(p(q)) \cdot p'(q)
$$

So:

$$
1 = -F'(p(q)) \cdot p'(q)
$$

Solve for $p'(q)$  :

$$
p'(q) = -\frac{1}{F'(p(q))}
$$

This matches our previous result, reinforcing confidence in the solution.

---

### Step 5: Verify with Examples

**Uniform Distribution on \[0, 1\]:** $F(\theta) = \theta$  , $F'(\theta) = 1$  .

$$
q(p) = 1 - F(p) = 1 - p
$$
 
$$
p(q) = 1 - q
$$
 
$$
p'(q) = -1
$$

Check: $F'(p(q)) = F'(1 - q) = 1$  , so:

$$
-\frac{1}{F'(p(q))} = -\frac{1}{1} = -1
$$

Matches perfectly.

**Distribution $F(\theta) = \theta^2$  on \[0, 1\]:** $F'({\theta}) = 2\theta$  .

$$
q(p) = 1 - p^2
$$
 
$$
p(q) = (1 - q)^{1/2}
$$
 
$$
p'(q) = \frac{1}{2} (1 - q)^{-1/2} \cdot (-1) = -\frac{1}{2 (1 - q)^{1/2}}
$$

Check: $p(q) = (1 - q)^{1/2}$  , so $F'(p(q)) = 2 \cdot (1 - q)^{1/2}$  , then:

$$
-\frac{1}{F'(p(q))} = -\frac{1}{2 (1 - q)^{1/2}}
$$

This matches $p'(q)$  , confirming consistency.

---

### Step 6: Evaluate the Options

The options are:

- (a) $p'(q) = -\frac{1}{F'(p(q))}$
- (b) $p'(q) = -F'(p(q))$
- (c) $p'(q) = -\frac{1}{F'(q)}$
- (d) $p'(q) = -F'(q)$

Our derivation gives $p'(q) = -\frac{1}{F'(p(q))}$  , matching (a). Let’s test alternatives:

- **Option (b):** In the second example, $F'(p(q)) = 2 (1 - q)^{1/2}$  , so $-F'(p(q)) = -2 (1 - q)^{1/2}$  , but $p'(q) = -\frac{1}{2 (1 - q)^{1/2}}$  . These differ (e.g., at $q = 0.5$  , $-2 \sqrt{0.5} \approx -1.414$  , vs. $-\frac{1}{2 \sqrt{0.5}} \approx -0.707$  ).
- **Option (c):** $F'(q)$  implies $q$  is a valuation, but $q$  is quantity (0 to 1), not necessarily in $[\underline{\theta}, \overline{\theta}]$  . In the uniform case, $F'(q) = 1$  , so $-\frac{1}{F'(q)} = -1$  , which works, but in the second example, $F'(0.5) = 2 \cdot 0.5 = 1$  , giving $-1$ , while $p'(0.5) \approx -0.707$  . Inconsistent.
- **Option (d):** $-F'(q) = -2q$  in the second example; at $q = 0.5$  , $-2 \cdot 0.5 = -1$  , vs. $p'(0.5) \approx -0.707$  . Incorrect.

Only (a) holds consistently.

---

### Conclusion

The slope of the inverse demand function is:

$$
p'(q) = -\frac{1}{F'(p(q))}
$$

This corresponds to option (a), reflecting how price decreases as quantity increases, with the rate depending on the density of valuations at the price $p(q)$  . https://grok.com/chat/9d0949ff-6cb9-4434-9d8f-a8d73da47f52