---
title: Summation of Binomial Coefficients
source: https://chatgpt.com/c/67eb272a-53ac-8008-862e-92831c2be3f1
author:
  - "[[Cournot2]]"
published: 
created: 2025-04-01
description: ChatGPT conversation with 5 turns
tags:
  - clippings
  - imp
---
## ChatGPT

A well-known identity is:

$$
∑k=0m(−1)k(mk)2  =  {0,if m is odd,(−1)m2(mm2),if m is even.\sum_{k=0}^{m}(-1)^k \binom{m}{k}^2 \;=\;
\begin{cases}
0, & \text{if $m$ is odd},\\[6pt]
(-1)^{\tfrac{m}{2}}\binom{m}{\tfrac{m}{2}}, & \text{if $m$ is even}.
\end{cases}k=0∑m(−1)k(km)2=⎩⎨⎧0,(−1)2m(2mm),if m is odd,if m is even.
$$

In the problem, $m=2nm = 2nm=2n$ (which is certainly even). Hence,

$$
∑k=02n(−1)k(2nk)2  =  (−1)2n2(2n2n2)  =  (−1)n(2nn).\sum_{k=0}^{2n} (-1)^k \binom{2n}{k}^2 
\;=\; 
(-1)^{\tfrac{2n}{2}} \binom{2n}{\tfrac{2n}{2}}
\;=\;
(-1)^{n} \binom{2n}{n}.k=0∑2n(−1)k(k2n)2=(−1)22n(22n2n)=(−1)n(n2n).
$$

So the value of

$$
(2n0)2  −  (2n1)2  +  (2n2)2  −  …  +  (−1)2n(2n2n)2\binom{2n}{0}^2 \;-\;\binom{2n}{1}^2 \;+\;\binom{2n}{2}^2 \;-\;\dots\;+\;(-1)^{2n}\binom{2n}{2n}^2(02n)2−(12n)2+(22n)2−…+(−1)2n(2n2n)2
$$

is

$$
(−1)n(2nn).\boxed{(-1)^n \binom{2n}{n}}.(−1)n(n2n).
$$

---

## You

explain this identity then

---

## ChatGPT

One elegant way to explain the identity

$$
∑k=0m(−1)k(mk)2={0,if m is odd,(−1)m/2(mm/2),if m is even,\sum_{k=0}^{m} (-1)^k \binom{m}{k}^2 =
\begin{cases}
0, & \text{if } m \text{ is odd},\\[1mm]
(-1)^{m/2}\binom{m}{m/2}, & \text{if } m \text{ is even},
\end{cases}k=0∑m(−1)k(km)2={0,(−1)m/2(m/2m),if m is odd,if m is even,
$$

is by using generating functions. Here’s a step-by-step explanation:

---

### 1\. Consider a Product of Generating Functions

Look at the product

$$
(1+x)m(1−x)m.(1+x)^m (1-x)^m.(1+x)m(1−x)m.
$$

Expanding each factor, we have:

- $(1+x)m=∑k=0m(mk)xk(1+x)^m = \sum_{k=0}^m \binom{m}{k} x^k(1+x)m=∑k=0m(km)xk$ ,
- $(1−x)m=∑j=0m(mj)(−1)jxj(1-x)^m = \sum_{j=0}^m \binom{m}{j} (-1)^j x^j(1−x)m=∑j=0m(jm)(−1)jxj$ .

When you multiply these two series, you get

$$
(1+x)m(1−x)m=∑k=0m∑j=0m(mk)(mj)(−1)jxk+j.(1+x)^m (1-x)^m = \sum_{k=0}^m \sum_{j=0}^m \binom{m}{k}\binom{m}{j} (-1)^j x^{k+j}.(1+x)m(1−x)m=k=0∑mj=0∑m(km)(jm)(−1)jxk+j.
$$

---

### 2\. Focus on the Coefficient of xmx^m

The coefficient of $xmx^mxm$ in the product is obtained by summing over all pairs $(k,j)(k, j)(k,j)$ such that $k+j=mk+j = mk+j=m$ :

$$
Coefficient of xm=∑k=0m(mk)(mm−k)(−1)m−k.\text{Coefficient of } x^m = \sum_{k=0}^{m} \binom{m}{k}\binom{m}{m-k} (-1)^{m-k}.Coefficient of xm=k=0∑m(km)(m−km)(−1)m−k.
$$

Notice that $(mm−k)=(mk)\binom{m}{m-k} = \binom{m}{k}(m−km)=(km)$ . Thus, the coefficient becomes

$$
∑k=0m(mk)2(−1)m−k.\sum_{k=0}^{m} \binom{m}{k}^2 (-1)^{m-k}.k=0∑m(km)2(−1)m−k.
$$

If we factor out a common $(−1)m(-1)^m(−1)m$ , this expression can be written as

$$
(−1)m∑k=0m(−1)k(mk)2.(-1)^m \sum_{k=0}^{m} (-1)^k \binom{m}{k}^2.(−1)mk=0∑m(−1)k(km)2.
$$

---

### 3\. Compare with the Alternate Expansion

On the other hand, note that

$$
(1+x)m(1−x)m=(1−x2)m.(1+x)^m (1-x)^m = (1-x^2)^m.(1+x)m(1−x)m=(1−x2)m.
$$

Expanding $(1−x2)m(1-x^2)^m(1−x2)m$ gives

$$
(1−x2)m=∑i=0m(mi)(−1)ix2i.(1-x^2)^m = \sum_{i=0}^{m} \binom{m}{i} (-1)^i x^{2i}.(1−x2)m=i=0∑m(im)(−1)ix2i.
$$

Observe that in this expansion, only even powers of $xxx$ appear. This means:

- If $mmm$ is **odd**, there is **no** $xmx^mxm$ term (because $mmm$ is odd and cannot be written as $2i2i2i$ ).
- If $mmm$ is **even**, say $m=2im = 2im=2i$ , the coefficient of $xmx^mxm$ (which is $x2ix^{2i}x2i$ ) is
	$$
	(mm/2)(−1)m/2.\binom{m}{m/2} (-1)^{m/2}.(m/2m)(−1)m/2.
	$$

---

### 4\. Equate the Two Expressions for the Coefficient of xmx^m

We now have two expressions for the coefficient of $xmx^mxm$ :

1. From the product expansion:
	$$
	(−1)m∑k=0m(−1)k(mk)2.(-1)^m \sum_{k=0}^{m} (-1)^k \binom{m}{k}^2.(−1)mk=0∑m(−1)k(km)2.
	$$
2. From the expansion of $(1−x2)m(1-x^2)^m(1−x2)m$ :
	- $000$ if $mmm$ is odd,
	- $(mm/2)(−1)m/2\binom{m}{m/2} (-1)^{m/2}(m/2m)(−1)m/2$ if $mmm$ is even.

Thus, equating these, we have:

- **For odd $mmm$ :**
	$$
	(−1)m∑k=0m(−1)k(mk)2=0.(-1)^m \sum_{k=0}^{m} (-1)^k \binom{m}{k}^2 = 0.(−1)mk=0∑m(−1)k(km)2=0.
	$$
	Multiplying both sides by $(−1)m(-1)^m(−1)m$ (which is nonzero) gives
	$$
	∑k=0m(−1)k(mk)2=0.\sum_{k=0}^{m} (-1)^k \binom{m}{k}^2 = 0.k=0∑m(−1)k(km)2=0.
	$$
- **For even $mmm$ :**
	$$
	(−1)m∑k=0m(−1)k(mk)2=(−1)m/2(mm/2).(-1)^m \sum_{k=0}^{m} (-1)^k \binom{m}{k}^2 = (-1)^{m/2} \binom{m}{m/2}.(−1)mk=0∑m(−1)k(km)2=(−1)m/2(m/2m).
	$$
	Multiplying both sides by $(−1)m(-1)^m(−1)m$ (or, equivalently, rewriting the sign) yields
	$$
	∑k=0m(−1)k(mk)2=(−1)m−m/2(mm/2)=(−1)m/2(mm/2).\sum_{k=0}^{m} (-1)^k \binom{m}{k}^2 = (-1)^{m - m/2}\binom{m}{m/2} = (-1)^{m/2}\binom{m}{m/2}.k=0∑m(−1)k(km)2=(−1)m−m/2(m/2m)=(−1)m/2(m/2m).
	$$

---

### 5\. Final Identity

Thus, we arrive at the final identity:

$$
∑k=0m(−1)k(mk)2={0,if m is odd,(−1)m/2(mm/2),if m is even.\sum_{k=0}^{m} (-1)^k \binom{m}{k}^2 =
\begin{cases}
0, & \text{if } m \text{ is odd},\\[1mm]
(-1)^{m/2}\binom{m}{m/2}, & \text{if } m \text{ is even}.
\end{cases}k=0∑m(−1)k(km)2={0,(−1)m/2(m/2m),if m is odd,if m is even.
$$

This explanation shows how generating functions and comparing coefficients lead us directly to the result.

---

## You

cant understand shit in it

---

## ChatGPT

Let's break it down into simpler, more intuitive steps. We want to understand why

$$
∑k=0m(−1)k(mk)2={0,if m is odd,(−1)m/2(mm/2),if m is even.\sum_{k=0}^{m} (-1)^k \binom{m}{k}^2 =
\begin{cases}
0, & \text{if } m \text{ is odd},\\[1mm]
(-1)^{m/2}\binom{m}{m/2}, & \text{if } m \text{ is even}.
\end{cases}k=0∑m(−1)k(km)2={0,(−1)m/2(m/2m),if m is odd,if m is even.
$$

We'll use a method involving generating functions (polynomial expansions) but in a more step-by-step, plain language way.

---

### Step 1. Write Two Polynomial Expansions

1. **Expand $(1+x)m(1+x)^m(1+x)m$ :**
	This gives:
	$$
	(1+x)m=(m0)+(m1)x+(m2)x2+⋯+(mm)xm.(1+x)^m = \binom{m}{0} + \binom{m}{1}x + \binom{m}{2}x^2 + \dots + \binom{m}{m}x^m.(1+x)m=(0m)+(1m)x+(2m)x2+⋯+(mm)xm.
	$$
2. **Expand $(1−x)m(1-x)^m(1−x)m$ :**
	Here, every $xxx$ term comes with a minus sign:
	$$
	(1−x)m=(m0)−(m1)x+(m2)x2−⋯+(−1)m(mm)xm.(1-x)^m = \binom{m}{0} - \binom{m}{1}x + \binom{m}{2}x^2 - \dots + (-1)^m \binom{m}{m}x^m.(1−x)m=(0m)−(1m)x+(2m)x2−⋯+(−1)m(mm)xm.
	$$

---

### Step 2. Multiply the Two Expansions

When you multiply $(1+x)m(1+x)^m(1+x)m$ by $(1−x)m(1-x)^m(1−x)m$ , you are essentially multiplying every term from the first expansion with every term from the second. The result is:

$$
(1+x)m(1−x)m.(1+x)^m(1-x)^m.(1+x)m(1−x)m.
$$

A key observation is that multiplying these two expressions directly gives a simpler result:

$$
(1+x)m(1−x)m=(1−x2)m.(1+x)^m(1-x)^m = (1-x^2)^m.(1+x)m(1−x)m=(1−x2)m.
$$

---

### Step 3. Look at the Coefficient of a Specific Power

The trick is to look at the coefficient (the number in front) of $xmx^mxm$ on both sides of the equality. The coefficient tells us the total “weight” of all terms that add up to $xmx^mxm$ .

1. **From the product of two expansions:**
	When you multiply the two series, a typical term looks like:
	$$
	(mk)xk×(−1)j(mj)xj=(−1)j(mk)(mj)xk+j.\binom{m}{k} x^k \times (-1)^{j} \binom{m}{j} x^j = (-1)^j \binom{m}{k} \binom{m}{j} x^{k+j}.(km)xk×(−1)j(jm)xj=(−1)j(km)(jm)xk+j.
	$$
	To get $xmx^mxm$ , you need $k+j=mk + j = mk+j=m$ . If you set $j=m−kj = m - kj=m−k$ , the coefficient for $xmx^mxm$ becomes:
	$$
	∑k=0m(mk)(mm−k)(−1)m−k.\sum_{k=0}^{m} \binom{m}{k} \binom{m}{m-k} (-1)^{m-k}.k=0∑m(km)(m−km)(−1)m−k.
	$$
	Notice that $(mm−k)=(mk)\binom{m}{m-k} = \binom{m}{k}(m−km)=(km)$ , so this sum is:
	$$
	∑k=0m(−1)m−k(mk)2.\sum_{k=0}^{m} (-1)^{m-k} \binom{m}{k}^2.k=0∑m(−1)m−k(km)2.
	$$
	If you factor out a common sign factor $(−1)m(-1)^m(−1)m$ (because $(−1)m−k=(−1)m(−1)k(-1)^{m-k} = (-1)^m (-1)^k(−1)m−k=(−1)m(−1)k$ ), it becomes:
	$$
	(−1)m∑k=0m(−1)k(mk)2.(-1)^m \sum_{k=0}^{m} (-1)^k \binom{m}{k}^2.(−1)mk=0∑m(−1)k(km)2.
	$$
	Let’s call our sum $SSS$ . Then we have:
	$$
	Coefficient from the product=(−1)mS.\text{Coefficient from the product} = (-1)^m S.Coefficient from the product=(−1)mS.
	$$
2. **From the simpler expansion $(1−x2)m(1-x^2)^m(1−x2)m$ :**
	Now expand $(1−x2)m(1-x^2)^m(1−x2)m$ . Notice that $xxx$ only appears as $x2x^2x2$ , so only even powers of $xxx$ will be present. Its expansion is:
	$$
	(1−x2)m=(m0)−(m1)x2+(m2)x4−… .(1-x^2)^m = \binom{m}{0} - \binom{m}{1} x^2 + \binom{m}{2} x^4 - \dots.(1−x2)m=(0m)−(1m)x2+(2m)x4−….
	$$
	- If $mmm$ is **odd**, there is no term with $xmx^mxm$ because $mmm$ (an odd number) can’t be written as $2i2i2i$ for any integer $iii$ . So, the coefficient of $xmx^mxm$ is $000$ .
	- If $mmm$ is **even**, say $m=2im = 2im=2i$ , then the $xm=x2ix^m = x^{2i}xm=x2i$ term comes from the $iii$ th term in the expansion:
		$$
		Coefficient=(mi)(−1)i=(mm/2)(−1)m/2.\text{Coefficient} = \binom{m}{i} (-1)^i = \binom{m}{m/2} (-1)^{m/2}.Coefficient=(im)(−1)i=(m/2m)(−1)m/2.
		$$

---

### Step 4. Equate the Coefficients

Since the two different ways of expanding the same product must give the same coefficient for $xmx^mxm$ , we have:

- **If $mmm$ is odd:**
	$$
	(−1)mS=0.(-1)^m S = 0.(−1)mS=0.
	$$
	Since $(−1)m(-1)^m(−1)m$ is not zero, it forces:
	$$
	S=0.S = 0.S=0.
	$$
- **If $mmm$ is even:**
	$$
	(−1)mS=(−1)m/2(mm/2).(-1)^m S = (-1)^{m/2} \binom{m}{m/2}.(−1)mS=(−1)m/2(m/2m).
	$$
	Multiplying both sides by $(−1)−m(-1)^{-m}(−1)−m$ (which just flips the sign if needed) gives:
	$$
	S=(−1)m/2(mm/2).S = (-1)^{m/2} \binom{m}{m/2}.S=(−1)m/2(m/2m).
	$$

Remember, $SSS$ is exactly the sum:

$$
S=∑k=0m(−1)k(mk)2.S = \sum_{k=0}^{m} (-1)^k \binom{m}{k}^2.S=k=0∑m(−1)k(km)2.
$$

---

### Final Summary

- **When $mmm$ is odd:** The sum is $000$ .
- **When $mmm$ is even:** The sum is $(−1)m/2(mm/2)(-1)^{m/2}\binom{m}{m/2}(−1)m/2(m/2m)$ .

This step-by-step matching of coefficients is the key idea. By writing the same product in two different ways, we can “read off” the sum we are interested in. The method may seem a bit abstract at first, but it’s all about comparing the parts (coefficients) of the same polynomial written in two different ways.

I hope this clearer, simpler breakdown helps! Let me know if you'd like any part explained further. https://chatgpt.com/c/67eb272a-53ac-8008-862e-92831c2be3f1