$f(x + h) = f(x) + f'(x)h + f''(x) \frac{h^{2}}{2!} + \dots$


$f(x + h) = f(x) + f'(x)h + f''(x) \frac{h^{2}}{2!} + f'''(x) \frac{h^{3}}{3!} + f^{(4)}(x) \frac{h^{4}}{4!}+ \dots$



$f(x) = f(0) + f'(0)x + f''(0) \frac{x^{2}}{2!} + f'''(0) \frac{x^{3}}{3!} + f^{(4)}(0) \frac{x^{4}}{4!} + \dots$

$(1 + x)^{r} = 1 + r x + \frac{r(r - 1)}{2!} x^2 + \frac{r(r - 1)(r - 2)}{3!} x^3 + \dots$$

$f(x) = \frac{a_0}{2} + \sum_{n=1}^{\infty} \left( a_n \cos(nx) + b_n \sin(nx) \right)$$


$f(x) = f(0) + f'(0)({1:x}) + \frac{{0:f}''(0)({1:x})^2}{2!} + \frac{{0:f}'''(0)({1:x})^3}{3!} + \dots$$

$(1 + x)^{r} = 1 + (r)({0:x}) + \frac{({1:r})({1:r} - 1)({0:x})^2}{2!} + \frac{({1:r})({1:r} - 1)({1:r} - 2)({0:x})^3}{3!} + \dots$
